Prove step_spec

doc/coq/.CoqMakefile.d
@@ -7,18 +7,21 @@ simple/ALinking.vos simple/ALinking.vok simple/ALinking.required_vos: simple/ALi
 simple/Abstract.vo simple/Abstract.glob simple/Abstract.v.beautified simple/Abstract.required_vo: simple/Abstract.v simple/Concrete.vo
 simple/Abstract.vio: simple/Abstract.v simple/Concrete.vio
 simple/Abstract.vos simple/Abstract.vok simple/Abstract.required_vos: simple/Abstract.v simple/Concrete.vos
+simple/Bound.vo simple/Bound.glob simple/Bound.v.beautified simple/Bound.required_vo: simple/Bound.v simple/Abstract.vo simple/Concrete.vo
+simple/Bound.vio: simple/Bound.v simple/Abstract.vio simple/Concrete.vio
+simple/Bound.vos simple/Bound.vok simple/Bound.required_vos: simple/Bound.v simple/Abstract.vos simple/Concrete.vos
 simple/Concrete.vo simple/Concrete.glob simple/Concrete.v.beautified simple/Concrete.required_vo: simple/Concrete.v simple/Syntax.vo
 simple/Concrete.vio: simple/Concrete.v simple/Syntax.vio
 simple/Concrete.vos simple/Concrete.vok simple/Concrete.required_vos: simple/Concrete.v simple/Syntax.vos
-simple/Equiv.vo simple/Equiv.glob simple/Equiv.v.beautified simple/Equiv.required_vo: simple/Equiv.v simple/Abstract.vo simple/Concrete.vo
-simple/Equiv.vio: simple/Equiv.v simple/Abstract.vio simple/Concrete.vio
-simple/Equiv.vos simple/Equiv.vok simple/Equiv.required_vos: simple/Equiv.v simple/Abstract.vos simple/Concrete.vos
+simple/Equiv.vo simple/Equiv.glob simple/Equiv.v.beautified simple/Equiv.required_vo: simple/Equiv.v simple/Bound.vo
+simple/Equiv.vio: simple/Equiv.v simple/Bound.vio
+simple/Equiv.vos simple/Equiv.vok simple/Equiv.required_vos: simple/Equiv.v simple/Bound.vos
 simple/Linking.vo simple/Linking.glob simple/Linking.v.beautified simple/Linking.required_vo: simple/Linking.v simple/Concrete.vo
 simple/Linking.vio: simple/Linking.v simple/Concrete.vio
 simple/Linking.vos simple/Linking.vok simple/Linking.required_vos: simple/Linking.v simple/Concrete.vos
-simple/Sound.vo simple/Sound.glob simple/Sound.v.beautified simple/Sound.required_vo: simple/Sound.v simple/Equiv.vo simple/ALinking.vo simple/Linking.vo
-simple/Sound.vio: simple/Sound.v simple/Equiv.vio simple/ALinking.vio simple/Linking.vio
-simple/Sound.vos simple/Sound.vok simple/Sound.required_vos: simple/Sound.v simple/Equiv.vos simple/ALinking.vos simple/Linking.vos
+simple/Sound.vo simple/Sound.glob simple/Sound.v.beautified simple/Sound.required_vo: simple/Sound.v simple/Bound.vo simple/ALinking.vo simple/Linking.vo
+simple/Sound.vio: simple/Sound.v simple/Bound.vio simple/ALinking.vio simple/Linking.vio
+simple/Sound.vos simple/Sound.vok simple/Sound.required_vos: simple/Sound.v simple/Bound.vos simple/ALinking.vos simple/Linking.vos
 simple/Syntax.vo simple/Syntax.glob simple/Syntax.v.beautified simple/Syntax.required_vo: simple/Syntax.v tactics/sflib.vo
 simple/Syntax.vio: simple/Syntax.v tactics/sflib.vio
 simple/Syntax.vos simple/Syntax.vok simple/Syntax.required_vos: simple/Syntax.v tactics/sflib.vos
