doc/coq/simple/Equiv.v
@@ -1,381 +1,471 @@
-From Simple Require Export Abstract.
-From Simple Require Export Concrete.
+From Simple Require Export Bound.
 
-Ltac lebt x :=
-  apply leb_trans with (t' := x);
-  try assumption; try apply tick_lt; try apply leb_refl.
+Generalizable Variables T.
 
-Generalizable Variables T aT TT aTT.
-
-Definition time_bound_C `{TotalOrder T} C t :=
-  forall t', supp_C C t' -> leb t' t = true.
-
-Definition time_bound_m `{TotalOrder T} m t :=
-  forall t', supp_m m t' -> leb t' t = true.
-
-Definition time_bound_v `{TotalOrder T} v t :=
-  match v with
-  | Closure _ _ C => time_bound_C C t
+Lemma read_top `{Eq T} :
+  forall a b t,
+  read (a ++ b) t = 
+  match read a t with
+  | None => read b t
+  | Some _ => read a t
   end.
-
-Definition time_bound_V `{TotalOrder T} V t :=
-  match V with
-  | EVal ev => time_bound_v ev t
-  | MVal mv => time_bound_C mv t
-  end.
-
-Definition time_bound_ρ `{TotalOrder T} (ρ : config T) :=
-  match ρ with
-  | Cf _ C m t =>
-    time_bound_C C t /\ time_bound_m m t
-  | Rs V m t =>
-    time_bound_V V t /\ time_bound_m m t
-  end.
-
-Lemma not_le_lt `{TotalOrder T} :
-  forall (p : T) t,
-    (leb p t = false) <-> (t < p).
 Proof.
-  intros; unfold "<"; red; split; intros NLE;
+  induction a; ii; ss;
+  repeat des_goal; repeat des_hyp; clarify;
+  repeat rw; reflexivity.
+Qed.
+
+Lemma app_same `{Eq T} :
+  forall l l' m m'
+    (SAMEl : same l l')
+    (SAMEm : same m m'),
+    same (l ++ m) (l' ++ m').
+Proof.
+  pose proof read_top.
+  ii. repeat rw. unfold same in SAMEl.
+  repeat des_goal; clarify;
   repeat match goal with
-  | H : _ /\ _ |- _ => destruct H
-  | |- context [leb ?p ?t] =>
-    let RR := fresh "RR" in
-    destruct (leb p t) eqn:RR
-  | |- context [eqb ?p ?t] =>
-    let RR := fresh "RR" in
-    destruct (eqb p t) eqn:RR
-  | H : context [leb ?p ?t] |- _ =>
-    match goal with
-    | _ : leb p t = true |- _ => idtac
-    | _ : leb p t = false |- _ => idtac
-    | _ =>
-      let RR := fresh "RR" in
-      destruct (leb p t) eqn:RR
-    end
+  | H : read _ _ = _ |- _ => symmetry in H
   end;
-  try rewrite eqb_eq in *;
-  try rewrite eqb_neq in *; subst;
-  try rewrite leb_refl in *;
-  clarify; exfalso; eauto using leb_sym.
-  pose proof leb_or as contra.
-  specialize (contra p t).
-  rewrite NLE in *. rewrite RR in *. clarify.
-Qed.
-
-Lemma time_bound_or_not `{TotalOrder T} :
-  forall (p : T) t,
-    (p < t) \/ ~(p < t).
-Proof.
-  intros.
-  rewrite <- not_le_lt.
-  destruct (leb t p); eauto.
-Qed.
-
-Lemma time_increase `{time T} :
-  forall e C m t cf' (EVAL : {|(Cf e C m t) ~> cf'|}),
-    match cf' with
-    | Cf _ _ _ t'
-    | Rs _ _ t' => leb t t' = true
-    end.
-Proof.
-  intros.
-  remember (Cf e C m t) as cf. ginduction EVAL;
-  intros; clarify; try apply leb_refl; eauto 2;
-  try (exploit IHEVAL3; eauto 1);
-  try (exploit IHEVAL2; eauto 1);
-  try (exploit IHEVAL1; eauto 1);
-  try (exploit IHEVAL; eauto 1); intros;
-  try lebt t';
-  try lebt t_f;
-  try lebt t_a;
+  first [rewrite SAMEl in * | rewrite <- SAMEl in *];
   match goal with
-  | _ : context [tick ?C ?m ?t ?x ?v] |- _ =>
-    lebt (tick C m t x v)
+  | _ : ?a = read ?l ?t, _ : ?b = read ?l ?t |- _ =>
+    assert (a = b); clarify; repeat rw; eauto
   end.
 Qed.
 
-Lemma relax_ctx_bound `{time T} :
-  forall C t1 t2 (BOUND : time_bound_C C t1) (LE : leb t1 t2 = true),
-         time_bound_C C t2.
+Lemma disj_reflect `{Eq T} :
+  forall m m',
+  (forall t (READ : None <> read m t), None = read m' t) <->
+  (forall t (READ : None <> read m' t), None = read m t).
 Proof.
-  induction C; unfold time_bound_C;
-  intros; ss; des; clarify;
-  match goal with
-  | H : supp_C ?C ?t |- _ =>
-    match goal with
-    | H : context [time_bound_C C _] |- _ => eapply H; eauto
-    end
-  | _ => idtac
-  end; try red; intros; try apply BOUND; eauto.
-  - lebt t1. apply BOUND. left; eauto.
+  induction m; ii; ss;
+  repeat des_goal; clarify.
+  split; intros IN ? ?; try des_goal; try des_hyp; clarify.
+  - rewrite eqb_eq in *; clarify.
+    exfalso. apply READ. apply IN. rewrite t_refl.
+    red; ii; clarify.
+  - assert (forall t, None <> read m' t -> None = read m t); eauto.
+    rewrite <- IHm.
+    ii. apply IN. red; ii; des_hyp; clarify.
+  - rewrite eqb_eq in *; clarify.
+    specialize (IN t0). rewrite t_refl in *.
+    destruct (read m' t0); eauto.
+    assert (None = Some e); clarify.
+    apply IN; red; ii; clarify.
+  - assert (forall t, None <> read m t -> None = read m' t); eauto.
+    rewrite IHm.
+    ii. specialize (IN t1). apply IN in READ0.
+    des_hyp; clarify.
 Qed.
 
-Lemma relax_p_bound `{time T} :
-  forall p t1 t2 (BOUND : p < t1) (LE : leb t1 t2 = true),
-    p < t2.
+Lemma app_disj_same `{Eq T} :
+  forall m m' (DISJ : forall t (READ : None <> read m t), None = read m' t),
+  same (m ++ m') (m' ++ m).
 Proof.
-  intros. destruct BOUND as [? EQ]. split.
-  - lebt t1.
-  - rewrite eqb_neq in *. red; intros.
-    subst. apply EQ. apply leb_sym; eauto.
+  induction m; ii; ss.
+  - rewrite app_nil_r. eauto.
+  - des_goal.
+    assert (None = read m' t0).
+    apply DISJ. rewrite t_refl. red; ii; clarify.
+    des_goal; clarify.
+    + rewrite eqb_eq in *; clarify.
+      clear IHm DISJ.
+      ginduction m'; ii; ss. rewrite t_refl. eauto.
+      repeat des_hyp; clarify; eauto.
+    + assert (read (m' ++ (t0, e) :: m) t = read (m' ++ m) t) as RR.
+      {
+        clear H0 v DISJ IHm.
+        ginduction m'; ii; ss. rw. eauto.
+        repeat des_goal; clarify; eauto.
+      }
+      rewrite RR.
+      apply IHm. ii. apply DISJ.
+      red; ii. repeat des_hyp; clarify.
 Qed.
 
-Lemma relax_mem_bound `{time T} :
-  forall m t1 t2 (BOUND : time_bound_m m t1) (LE : leb t1 t2 = true),
-         time_bound_m m t2.
+Lemma eq_node_neq `{Eq T} :
+  forall n n', eq_node n n' = false <-> n <> n'.
 Proof.
-  induction m; unfold time_bound_m;
-  intros; ss; repeat des_hyp; clarify.
-  lebt t1. apply BOUND. eauto.
+  assert (eq_node = eqb) as RR. reflexivity.
+  rewrite RR in *. exact eqb_neq.
 Qed.
 
-Lemma time_bound_addr `{time T} :
-  forall C x t (BOUND : time_bound_C C t),
+Lemma same_comm `{Eq T} :
+  forall m m',
+  same m m' <-> same m' m.
+Proof.
+  intros; unfold same; split; ii; rw; eauto.
+Qed.
+
+Lemma same_trans `{Eq T} :
+  forall m m' m'' (SAME : same m m') (SAME' : same m' m''),
+  same m m''.
+Proof.
+  ii. unfold same in *. rewrite SAME. rewrite SAME'. eauto.
+Qed.
+
+Inductive edge T :=
+  | Ex (nC : node T) (x : ID) (ntx : node T)
+  | EM (nC : node T) (M : ID) (nCM : node T)
+  | Ev (nt : node T) (v : value) (nCv : node T)
+.
+
+Arguments Ex {T}.
+Arguments EM {T}.
+Arguments Ev {T}.
+
+Definition eq_val (v v' : value) :=
+  match v, v' with
+  | v_fn x e, v_fn x' e' => eqb x x' && eqb e e'
+  end.
+
+Lemma eq_val_eq :
+  forall v v', eq_val v v' = true <-> v = v'.
+Proof.
+  ii. unfold eq_val.
+  repeat des_goal; try rewrite eqb_ID_eq in *; clarify.
+  rewrite eq_tm_eq. split; ii; clarify.
+  rewrite eqb_ID_neq in *.
+  split; ii; clarify.
+Qed.
+
+#[export] Instance EqVal : Eq value :=
+  { eqb := eq_val; eqb_eq := eq_val_eq; }.
+
+Lemma eq_val_neq :
+  forall v v', eq_val v v' = false <-> v <> v'.
+Proof.
+  assert (eq_val = eqb) as RR. eauto.
+  rewrite RR. exact eqb_neq.
+Qed.
+
+Definition eq_edge `{Eq T} (e e' : edge T) :=
+  match e, e' with
+  | Ex nC x ntx, Ex nC' x' ntx' =>
+    eqb nC nC' && eqb x x' && eqb ntx ntx'
+  | EM nC M nCM, EM nC' M' nCM' =>
+    eqb nC nC' && eqb M M' && eqb nCM nCM'
+  | Ev nt v nCv, Ev nt' v' nCv' =>
+    eqb nt nt' && eqb v v' && eqb nCv nCv'
+  | _, _ => false
+  end.
+
+Lemma eq_edge_eq `{Eq T} :
+  forall e e', eq_edge e e' = true <-> e = e'.
+Proof.
+  ii. unfold eq_edge.
+  repeat des_goal; repeat des_hyp;
+  try rewrite eqb_ID_eq in *; 
+  try rewrite eqb_ID_neq in *;
+  try rewrite eq_node_eq in *;
+  try rewrite eq_node_neq in *;
+  try rewrite eq_val_eq in *;
+  try rewrite eq_val_neq in *;
+  split; ii; clarify.
+Qed.
+
+#[export] Instance EqEdge `{Eq T} : Eq (edge T) :=
+  { eqb := eq_edge; eqb_eq := eq_edge_eq; }.
+
+Lemma eq_edge_neq `{Eq T} :
+  forall e e', eq_edge e e' = false <-> e <> e'.
+Proof.
+  assert (eq_edge = eqb) as RR. eauto.
+  rewrite RR. exact eqb_neq.
+Qed.
+
+Definition valid_edge `{Eq T} (m : memory T) (e : edge T) :=
+  match e with
+  | Ex (Ctx C) x (Ptr tx) =>
     match addr_x C x with
-    | None => True
-    | Some addr => leb addr t = true
-    end.
-Proof.
-  induction C; unfold time_bound_C; intros; simpl in *; eauto;
-  repeat des_goal; repeat des_hyp; clarify;
-  match goal with
-  | IH : forall _ t, _ |- _ =>
-    match type of IH with
-    | context [addr_x ?C _] =>
-      match goal with
-      | RR : addr_x C ?x = _ |- _ =>
-        specialize (IH x t);
-        rewrite RR in IH;
-        apply IH; red; intros
-      end
+    | Some t => t = tx
+    | None => False
     end
-  | _ => idtac
-  end; apply BOUND; eauto.
-Qed.
-
-Lemma time_bound_read `{time T} :
-  forall m t addr (BOUND : time_bound_m m t),
-    match read m addr with
-    | None => True
-    | Some v => time_bound_v v t
-    end.
-Proof.
-  induction m; intros; simpl; eauto;
-  repeat des_goal; repeat des_hyp; eauto;
-  try rewrite eqb_eq in *; clarify;
-  match goal with
-  | _ => 
-    unfold time_bound_m in *;
-    unfold time_bound_v;
-    des_goal; red; intros; simpl in *;
-    apply BOUND; eauto; fail
-  | RR : read ?m ?addr = Some ?v |- _ => 
-    specialize (IHm t addr);
-    rewrite RR in IHm;
-    apply IHm; red; intros; apply BOUND; simpl; eauto
-  end.
-Qed.
-
-Lemma time_bound_ctx_M `{time T} :
-  forall C M t (BOUND : time_bound_C C t),
+  | EM (Ctx C) M (Ctx CM) =>
     match ctx_M C M with
-    | None => True
-    | Some CM => time_bound_C CM t
-    end.
+    | Some C => C = CM
+    | None => False
+    end
+  | Ev (Ptr t) v (Ctx Cv) =>
+    exists ev, Some ev = read m t /\
+    match ev with
+    | Closure x e C =>
+      v = v_fn x e /\ C = Cv
+    end
+  | _ => False
+  end.
+
+Definition avalid_edge `{Eq T} (m : memory T) (e : edge T) :=
+  match e with
+  | Ex (Ctx C) x (Ptr tx) =>
+    match addr_x C x with
+    | Some t => t = tx
+    | None => False
+    end
+  | EM (Ctx C) M (Ctx CM) =>
+    match ctx_M C M with
+    | Some C => C = CM
+    | None => False
+    end
+  | Ev (Ptr t) v (Ctx Cv) =>
+    exists ev, In ev (aread m t) /\
+    match ev with
+    | Closure x e C =>
+      v = v_fn x e /\ C = Cv
+    end
+  | _ => False
+  end.
+
+Lemma same_valid_edge `{Eq T} :
+  forall e m m' (SAME : same m m')
+    (VALe : valid_edge m e),
+  valid_edge m' e.
 Proof.
-  induction C; unfold time_bound_C; intros; simpl in *; eauto;
+  ii. unfold valid_edge.
   repeat des_goal; repeat des_hyp; clarify;
+  ss; repeat des_hyp; clarify.
+  des. repeat des_hyp; clarify.
+  des; clarify.
+  exists (Closure x e C). eauto.
+  unfold same in SAME.
+  rewrite <- SAME. eauto.
+Qed.
+
+Lemma asame_avalid_edge `{Eq T} :
+  forall e m m' (SAME : asame m m')
+    (VALe : avalid_edge m e),
+  avalid_edge m' e.
+Proof.
+  ii. unfold avalid_edge.
+  repeat des_goal; repeat des_hyp; clarify;
+  ss; repeat des_hyp; clarify.
+  des. repeat des_hyp; clarify.
+  des; clarify.
+  exists (Closure x e C). eauto.
+  unfold asame in SAME.
+  rewrite <- SAME. eauto.
+Qed.
+
+Fixpoint Edges `{Eq T} (n : node T) (p : path T) :=
+  match p with
+  | Pnil => []
+  | Px x n' tl => Ex n x n' :: Edges n' tl
+  | PM M n' tl => EM n M n' :: Edges n' tl
+  | Pv v n' tl => Ev n v n' :: Edges n' tl
+  end.
+
+Lemma vpath_iff_vedge `{Eq T} :
+  forall p m n,
+    valid_path n m p <->
+    forall e (IN : In e (Edges n p)), valid_edge m e.
+Proof.
+  induction p; ii; ss; repeat des_goal; repeat des_hyp; clarify; des;
+  split; ii; des; clarify; ltac:(
+  let HH := fresh "HH" in
   match goal with
-  | IH : forall _ t, _ |- _ =>
-    match type of IH with
-    | context [ctx_M ?C _] =>
-      match goal with
-      | RR : ctx_M C ?M = _ |- _ =>
-        specialize (IH M t);
-        rewrite RR in IH;
-        apply IH; red; intros
-      end
-    end
+  | H : forall e, Ex ?n ?x ?n' = e \/ _ -> _ |- _ =>
+    specialize (H (Ex n x n')) as HH; 
+    exploit HH; eauto;
+    ii; ss; repeat des_hyp; clarify
+  | H : forall e, EM ?n ?M ?n' = e \/ _ -> _ |- _ =>
+    specialize (H (EM n M n')) as HH; 
+    exploit HH; eauto;
+    ii; ss; repeat des_hyp; clarify
+  | H : forall e, Ev ?n ?v ?n' = e \/ _ -> _ |- _ =>
+    specialize (H (Ev n v n')) as HH; 
+    exploit HH; eauto;
+    ii; ss; repeat des_hyp; clarify
   | _ => idtac
-  end; try apply BOUND; eauto.
+  end).
+  - ss; des_goal; clarify.
+  - rewrite IHp in *. eauto.
+  - split; try rewrite IHp; ii; eauto.
+  - ss; des_goal; clarify.
+  - rewrite IHp in *. eauto.
+  - split; try rewrite IHp; ii; eauto.
+  - ss. exists ev. 
+    des_goal; des; repeat split; clarify.
+  - des_hyp; des; clarify.
+    rewrite IHp in *; eauto.
+  - des. exists ev.
+    des_goal; des; repeat split; clarify.
+    rewrite IHp; ii; eauto.
 Qed.
 
-Lemma leb_t_neq_tick `{time T} :
-  forall C m x v (t' t : T) (LE : leb t' t = true),
-  eqb t' (tick C m t x v) = false.
+Lemma avpath_iff_avedge `{Eq T} :
+  forall p m n,
+    avalid_path n m p <->
+    forall e (IN : In e (Edges n p)), avalid_edge m e.
 Proof.
-  intros. refl_bool. intros contra.
-  rewrite eqb_eq in *.
-  assert (t <> tick C m t x v) as NEQ.
-  { rewrite <- eqb_neq. apply tick_lt. }
-  apply NEQ. apply leb_sym. 
-  - apply tick_lt.
-  - subst. eauto.
-Qed.
-
-Lemma time_bound_tick `{time T} :
-  forall C m t x v
-         (BOUNDv : time_bound_v v t)
-         (BOUNDm : time_bound_m m t),
-  time_bound_m ((tick C m t x v) !-> v; m) (tick C m t x v).
-Proof.
-  intros.
-  unfold time_bound_v in *.
-  unfold time_bound_m in *. des_hyp.
-  unfold time_bound_C in *.
-  ii; ss; des; clarify;
+  induction p; ii; ss; repeat des_goal; repeat des_hyp; clarify; des;
+  split; ii; des; clarify; ltac:(
+  let HH := fresh "HH" in
   match goal with
-  | |- leb ?t ?t = true => apply leb_refl
-  | H : supp_C ?C _, 
-    BD : forall _, supp_C ?C _ -> _
-    |- leb _ (tick _ _ ?t _ _) = true  =>
-    apply BD in H; lebt t
-  | H : supp_m ?m _,
-    BD : forall _, supp_m ?m _ -> _ 
-    |- leb _ (tick _ _ ?t _ _) = true =>
-    apply BD in H; lebt t
-  end.
+  | H : forall e, Ex ?n ?x ?n' = e \/ _ -> _ |- _ =>
+    specialize (H (Ex n x n')) as HH; 
+    exploit HH; eauto;
+    ii; ss; repeat des_hyp; clarify
+  | H : forall e, EM ?n ?M ?n' = e \/ _ -> _ |- _ =>
+    specialize (H (EM n M n')) as HH; 
+    exploit HH; eauto;
+    ii; ss; repeat des_hyp; clarify
+  | H : forall e, Ev ?n ?v ?n' = e \/ _ -> _ |- _ =>
+    specialize (H (Ev n v n')) as HH; 
+    exploit HH; eauto;
+    ii; ss; repeat des_hyp; clarify
+  | _ => idtac
+  end).
+  - ss; des_goal; clarify.
+  - rewrite IHp in *. eauto.
+  - split; try rewrite IHp; ii; eauto.
+  - ss; des_goal; clarify.
+  - rewrite IHp in *. eauto.
+  - split; try rewrite IHp; ii; eauto.
+  - ss. exists ev. 
+    des_goal; des; repeat split; clarify.
+  - des_hyp; des; clarify.
+    rewrite IHp in *; eauto.
+  - des. exists ev.
+    des_goal; des; repeat split; clarify.
+    rewrite IHp; ii; eauto.
 Qed.
 
-Lemma trans_m_update `{TotalOrder T} {TT} (α : T -> TT) :
-  forall m t t' v (BOUND : time_bound_m m t) (LT : t < t'),
-    trans_m α (t' !-> v; m) =
-    (α t' !-> trans_v α v; trans_m α m).
+Definition reachable `{Eq T} root m e :=
+  exists p,
+    valid_path root m p /\
+    In e (Edges root p).
+
+Definition lvertex `{Eq T} (e : edge T) :=
+  match e with
+  | Ex n _ _
+  | EM n _ _
+  | Ev n _ _ => n
+  end.
+
+Definition rvertex `{Eq T} (e : edge T) :=
+  match e with
+  | Ex _ _ n
+  | EM _ _ n
+  | Ev _ _ n => n
+  end.
+
+Lemma reachable_paste `{Eq T} :
+  forall n m e (REACH : reachable n m e)
+    e' (EXT : rvertex e = lvertex e')
+    (VAL : valid_edge m e'),
+    reachable n m e'.
 Proof.
-  intros.
-  assert (
-    forall l l' 
-      (IN : forall t'', (In t'' l' -> t' = t'' \/ In t'' l) /\ (In t'' l -> In t'' l')),
-    trans_m_aux α m l = trans_m_aux α m l') as RR.
-  {
-    intros. ginduction m; intros; simpl; eauto.
-    repeat des_goal; try rewrite eqb_eq in *; clarify;
-    try rewrite Inb_eq in *; try rewrite Inb_neq in *;
-    match goal with
-    | _ : In ?t _ |- _ = _ :: _ =>
-      specialize (IN t) as [L R];
-      match goal with
-      | H : In _ _ |- _ => apply R in H; contradict
-      end
-    | _ : In ?t _ |- _ :: _ = _ =>
-      specialize (IN t) as [L R];
-      match goal with
-      | H : In _ _ |- _ => apply L in H; des; clarify
-      end; rewrite <- not_le_lt in LT;
-      match goal with
-      | _ => contradict
-      | _ => 
-        assert (false = true);
-        try (rewrite <- LT; apply BOUND; s; auto);
-        contradict
-      end
-    | _ => erewrite IHm; eauto;
-      match goal with
-      | |- context [time_bound_m] => red; ii; apply BOUND; s; auto
-      | |- forall _, _ =>
-        ii; split; ii; ss; des; auto;
-        match goal with
-        | H : In ?t _ |- _ =>
-          specialize (IN t) as [L R];
-          first [apply L in H | apply R in H]; des; eauto
-        end
-      end
-    end.
-  }
-  unfold trans_m, update_m. s.
-  symmetry. erewrite RR; eauto.
-  intros; simpl; split; intros; eauto.
+  ii. unfold reachable in REACH. des.
+  ginduction p; ii; ss;
+  repeat des_hyp; clarify; des; clarify; ss;
+  destruct e'; ss;
+  repeat des_hyp; des; clarify;
+  repeat des_hyp; des; clarify;
+  try match goal with
+  | _ : rvertex _ = _ |- reachable _ _ ?e =>
+    exploit IHp; eauto;
+    try instantiate (1 := e); ss;
+    try match goal with
+    | _ : Some (Closure ?x ?e ?C) = _ |- _ =>
+      exists (Closure x e C)
+    | _ => rw
+    end; eauto;
+    unfold reachable; ii; des
+  end;
+  try match goal with
+  | _ : valid_path ?n _ ?p |- _ =>
+    solve [
+      exists (Px x n p); ss; rw; eauto|
+      exists (PM M n p); ss; rw; eauto]
+  | _ : Some (Closure ?x ?e _) = _,
+    _ : valid_path (Ctx ?C) _ ?p |- _ =>
+    solve [
+      exists (Pv (v_fn x e) (Ctx C) p);
+      ss; repeat split; eauto;
+      exists (Closure x e C); ss]
+  end.
+  - exists (Px x (Ptr t) (Pv (v_fn x0 e) (Ctx C0) Pnil)).
+    ss; rw. repeat split; eauto.
+    exists (Closure x0 e C0). eauto.
+  - exists (PM M (Ctx C) (Px x (Ptr t) Pnil)).
+    ss. repeat rw. repeat split; eauto.
+  - exists (PM M (Ctx C) (PM M0 (Ctx C1) Pnil)).
+    ss. repeat rw. repeat split; eauto.
+  - exists (Pv (v_fn x0 e) (Ctx C0) (Px x (Ptr t0) Pnil)).
+    ss. repeat split; eauto.
+    exists (Closure x0 e C0). rw. eauto.
+  - exists (Pv (v_fn x e) (Ctx C0) (PM M (Ctx C1) Pnil)).
+    ss. repeat split; eauto.
+    exists (Closure x e C0). rw. eauto.
 Qed.
 
-Lemma time_bound `{time T} :
-  forall e C m t cf'
-         (EVAL : {|(Cf e C m t) ~> cf'|})
-         (BOUND : time_bound_ρ (Cf e C m t)),
-    time_bound_ρ cf'.
+Lemma reachable_left `{Eq T} :
+  forall n m e (REACH : reachable n m e),
+    n = lvertex e \/
+    exists e', reachable n m e' /\ rvertex e' = lvertex e.
 Proof.
-  intros. remember (Cf e C m t) as cf.
-  ginduction EVAL; intros; simpl; clarify;
-  unfold time_bound_ρ in *; eauto; destruct BOUND;
-  split; try assumption;
-  match goal with
-  | RR : read ?m ?addr = Some _ |- _ =>
-    match goal with
-    | H : time_bound_m m ?t |- _ =>
-      pose proof (time_bound_read m t addr H);
-      rewrite RR in *; assumption
-    end
-  | RR : ctx_M ?C ?M = Some _ |- _ =>
-    let HINT := fresh "HINT" in
-    pose proof (time_bound_ctx_M C M) as HINT;
-    rewrite RR in HINT; apply HINT; eauto
-  | _ =>
-    repeat match goal with
-    | EVAL : {|(Cf ?e ?C ?m ?t) ~> ?cf|} |- _ =>
-      lazymatch goal with
-      | _ : leb t _ = true |- _ => fail
-      | _ => pose proof (time_increase e C m t cf EVAL); simpl in *
-      end
-    end
-  end;
-  repeat match goal with
-  | IH : forall e C m t, _ -> _ -> ?P /\ ?Q |- _ =>
-    edestruct IH; eauto;
-    match goal with
-    | _ : P |- _ => 
-      clear IH; unfold time_bound_v in *;
-      repeat des_goal; repeat des_hyp
-    | |- _ /\ _ => split;
-      match goal with
-      | |- time_bound_C ?C ?t =>
-        match goal with
-        | _ : time_bound_C C ?t' |- _ =>
-          apply relax_ctx_bound with (t1 := t'); assumption
-        end
-      | |- time_bound_m ?m ?t => assumption
-      end
-    end
-  end; subst;
-  try (edestruct IHEVAL3; eauto);
-  try (edestruct IHEVAL2; eauto);
-  repeat match goal with
-  | |- _ /\ _ => split
-  | |- time_bound_C ?C ?t =>
-    red; intros; simpl in *;
-    repeat match goal with
-    | H : _ \/ _ |- _ => destruct H; subst; try apply tick_lt
-    | _ : supp_C ?C ?t |- leb ?t _ = true =>
-      match goal with
-      | H : time_bound_C C ?t' |- _ =>
-        lebt t'; try apply H; eauto 3
-      end
-    end
-  | |- time_bound_m ?m ?t => 
-    first [assumption |
-    apply time_bound_tick; simpl; assumption]
-  end;
-  first [apply leb_refl | lebt t_a | lebt t'].
+  ii. unfold reachable in REACH. des.
+  ginduction p; ii; ss; repeat des_hyp; clarify;
+  des; clarify; ss; repeat des_hyp;
+  clarify; des; clarify; eauto;
+  exploit IHp; eauto; ii; des; clarify; right.
+  - exists (Ex (Ctx C) x (Ptr t0)).
+    split; ss.
+    exists (Px x (Ptr t0) Pnil). ss. repeat rw. eauto.
+  - exists e'.
+    split; ss.
+    unfold reachable in *. des.
+    exists (Px x (Ptr t0) p0).
+    ss. rw. eauto.
+  - exists (EM (Ctx C0) M (Ctx d)).
+    split; ss.
+    exists (PM M (Ctx d) Pnil). ss. repeat rw. eauto.
+  - exists e'.
+    split; ss.
+    unfold reachable in *. des.
+    exists (PM M (Ctx d) p0).
+    ss. rw. eauto.
+  - exists (Ev (Ptr t) (v_fn x e0) (Ctx C0)).
+    split; ss.
+    exists (Pv (v_fn x e0) (Ctx C0) Pnil). ss.
+    repeat split; eauto.
+    exists (Closure x e0 C0). ss.
+  - exists e'.
+    split; ss.
+    unfold reachable in *. des.
+    exists (Pv (v_fn x e0) (Ctx C0) p0).
+    ss. split; eauto.
+    exists (Closure x e0 C0). ss.
 Qed.
 
-Fixpoint remove_x {T} (C : dy_ctx T) x :=
-  match C with
-  | [||] => [||]
-  | dy_binde x' t C' =>
-    let C' := remove_x C' x in
-    if eqb_ID x x' then C' else dy_binde x' t C'
-  | dy_bindm M C' C'' =>
-    dy_bindm M C' (remove_x C'' x)
-  end.
-
-Fixpoint remove_M {T} (C : dy_ctx T) M :=
-  match C with
-  | [||] => [||]
-  | dy_binde x t C' =>
-    dy_binde x t (remove_M C' M)
-  | dy_bindm M' C' C'' =>
-    let C'' := remove_M C'' M in
-    if eqb_ID M M' then C'' else dy_bindm M' C' C''
-  end.
+Lemma reachable_eq_def `{Eq T} :
+  forall n m e,
+    reachable n m e <->
+    (valid_edge m e /\
+      (n = lvertex e \/
+      exists e', 
+        reachable n m e' /\
+        rvertex e' = lvertex e)).
+Proof.
+  ii. split; intros REACH; des; clarify.
+  - split. unfold reachable in *. des.
+    rewrite vpath_iff_vedge in REACH. eauto.
+    apply reachable_left. eauto.
+  - destruct e; ss; repeat des_hyp; clarify; des;
+    repeat des_hyp; des; clarify;
+    match goal with
+    | |- context [Ex _ ?x (Ptr ?t)] =>
+      exists (Px x (Ptr t) Pnil)
+    | |- context [EM _ ?M (Ctx ?C)] =>
+      exists (PM M (Ctx C) Pnil)
+    | |- context [Ev _ ?v (Ctx ?C)] =>
+      exists (Pv v (Ctx C) Pnil)
+    end; ss; try rw; eauto.
+    split; eauto.
+    exists (Closure x e C). eauto.
+  - eapply reachable_paste; eauto.
+Qed.
 
 Fixpoint remove_t `{Eq T} (m : memory T) t :=
   match m with
@@ -385,25 +475,153 @@ Fixpoint remove_t `{Eq T} (m : memory T) t :=
     if eqb t t' then tl else (t', v) :: tl
   end.
 
-Fixpoint reach_C `{Eq T} seenx seenM (C : dy_ctx T) :=
-  match C with
+Fixpoint reach_C `{Eq T} seenx seenM (Cout Cin : dy_ctx T) :=
+  match Cin with
   | [||] => []
-  | dy_binde x t C =>
-    if Inb x seenx then reach_C seenx seenM C
-    else t :: reach_C (x :: seenx) seenM C
-  | dy_bindm M C C' =>
-    if Inb M seenM then reach_C seenx seenM C
-    else reach_C [] [] C ++ reach_C seenx (M :: seenM) C'
+  | dy_binde x t Cin =>
+    if Inb x seenx then reach_C seenx seenM Cout Cin
+    else Ex (Ctx Cout) x (Ptr t) ::
+    reach_C (x :: seenx) seenM Cout Cin
+  | dy_bindm M Cout' Cin =>
+    if Inb M seenM then reach_C seenx seenM Cout Cin
+    else reach_C [] [] Cout' Cout' ++ 
+    EM (Ctx Cout) M (Ctx Cout') ::
+    reach_C seenx (M :: seenM) Cout Cin
   end.
+
+Fixpoint InL `{Eq T} (n : node T) (l : list (edge T)) :=
+  match l with
+  | [] => false
+  | e :: tl => eqb n (lvertex e) || InL n tl
+  end.
+
+Fixpoint InR `{Eq T} (n : node T) (l : list (edge T)) :=
+  match l with
+  | [] => false
+  | e :: tl => eqb n (rvertex e) || InR n tl
+  end.
+
+Lemma InL_In `{Eq T} :
+  forall l n, InL n l = true <-> exists e, In e l /\ n = lvertex e.
+Proof.
+  induction l; ii; ss; split; ii; 
+  repeat des_goal; repeat des_hyp; ss; des; clarify;
+  first [rewrite eq_node_eq in * | rewrite eq_node_neq in *];
+  clarify.
+  - exists a. eauto.
+  - rewrite IHl in *. des. clarify.
+    exists e. eauto.
+  - rewrite IHl. exists e. eauto.
+Qed.
+
+Lemma InL_nIn `{Eq T} :
+  forall l n, InL n l = false <-> forall e, ~ In e l \/ n <> lvertex e.
+Proof.
+  split; intros NIN.
+  - assert (InL n l <> true) as HINT.
+    { refl_bool. eauto. }
+    red in HINT. rewrite InL_In in HINT.
+    ii.
+    destruct (Inb e l) eqn:CASEIn;
+    destruct (eqb n (lvertex e)) eqn:CASEv;
+    try rewrite Inb_eq in *;
+    try rewrite eqb_eq in *;
+    try rewrite Inb_neq in *;
+    try rewrite eqb_neq in *;
+    clarify; eauto.
+    exfalso. apply HINT. exists e. eauto.
+  - refl_bool. ii.
+    rewrite InL_In in *. des.
+    specialize (NIN e). des; eauto.
+Qed.
+
+Lemma InR_In `{Eq T} :
+  forall l n, InR n l = true <-> exists e, In e l /\ n = rvertex e.
+Proof.
+  induction l; ii; ss; split; ii; 
+  repeat des_goal; repeat des_hyp; ss; des; clarify;
+  first [rewrite eq_node_eq in * | rewrite eq_node_neq in *];
+  clarify.
+  - exists a. eauto.
+  - rewrite IHl in *. des. clarify.
+    exists e. eauto.
+  - rewrite IHl. exists e. eauto.
+Qed.
+
+Lemma InR_nIn `{Eq T} :
+  forall l n, InR n l = false <-> forall e, ~ In e l \/ n <> rvertex e.
+Proof.
+  split; intros NIN.
+  - assert (InR n l <> true) as HINT.
+    { refl_bool. eauto. }
+    red in HINT. rewrite InR_In in HINT.
+    ii.
+    destruct (Inb e l) eqn:CASEIn;
+    destruct (eqb n (rvertex e)) eqn:CASEv;
+    try rewrite Inb_eq in *;
+    try rewrite eqb_eq in *;
+    try rewrite Inb_neq in *;
+    try rewrite eqb_neq in *;
+    clarify; eauto.
+    exfalso. apply HINT. exists e. eauto.
+  - refl_bool. ii.
+    rewrite InR_In in *. des.
+    specialize (NIN e). des; eauto.
+Qed.
+
+Lemma InL_app_iff `{Eq T} :
+  forall n l1 l2,
+  InL n (l1 ++ l2) = true <-> InL n l1 = true \/ InL n l2 = true.
+Proof.
+  ii. split; ii; rewrite InL_In in *; des; clarify.
+  - rewrite in_app_iff in *. des.
+    left. exists e. eauto.
+    right. rewrite InL_In. exists e. eauto.
+  - exists e. rewrite in_app_iff. eauto.
+  - rewrite InL_In in *. des.
+    exists e. rewrite in_app_iff. eauto.
+Qed.
+
+Lemma InR_app_iff `{Eq T} :
+  forall n l1 l2,
+  InR n (l1 ++ l2) = true <-> InR n l1 = true \/ InR n l2 = true.
+Proof.
+  ii. split; ii; rewrite InR_In in *; des; clarify.
+  - rewrite in_app_iff in *. des.
+    left. exists e. eauto.
+    right. rewrite InR_In. exists e. eauto.
+  - exists e. rewrite in_app_iff. eauto.
+  - rewrite InR_In in *. des.
+    exists e. rewrite in_app_iff. eauto.
+Qed.
 
 Fixpoint reach_m_step `{Eq T} acc (m : memory T) :=
   match m with
   | [] => (acc, [])
   | (t, v) :: m =>
-    if Inb t acc then match v with
-    | Closure _ _ C =>
-      (reach_C [] [] C ++ acc, remove_t m t)
+    if InR (Ptr t) acc then match v with
+    | Closure x e C =>
+      (reach_C [] [] C C ++ 
+      Ev (Ptr t) (v_fn x e) (Ctx C) ::
+      acc, remove_t m t)
     end else match reach_m_step acc m with
+    | (acc, m) => (acc, (t, v) :: m)
+    end
+  end.
+
+Fixpoint areach_m_step `{Eq T} acc (m : memory T) :=
+  match m with
+  | [] => (acc, [])
+  | (t, v) :: m =>
+    if InR (Ptr t) acc then match v with
+    | Closure x e C =>
+      match areach_m_step acc m with
+      | (acc, m) =>
+        (reach_C [] [] C C ++
+        Ev (Ptr t) (v_fn x e) (Ctx C) ::
+        acc, m)
+      end
+    end else match areach_m_step acc m with
     | (acc, m) => (acc, (t, v) :: m)
     end
   end.
@@ -419,10 +637,7 @@ Fixpoint reach_m_aux `{Eq T} acc (m : memory T) fuel :=
     end
   end.
 
-Definition reach_m `{Eq T} init (m : memory T) :=
-  reach_m_aux init m (List.length m).
-
-Lemma remove_t_dec_len `{Eq T} :
+Lemma remove_t_dec `{Eq T} :
   forall (m : memory T) t,
   (List.length (remove_t m t)) <= (List.length m).
 Proof.
@@ -435,18 +650,85 @@ Proof.
   end.
 Qed.
 
-Lemma reach_m_step_dec_len `{Eq T} :
-  forall (m : memory T) acc,
+Lemma remove_t_read `{Eq T} :
+  forall (m : memory T) t,
+  None = read (remove_t m t) t.
+Proof.
+  induction m; ii; ss; repeat des_goal; repeat des_hyp; clarify.
+  rewrite eqb_eq in *; clarify. rewrite t_refl in *. clarify.
+Qed.
+
+Lemma remove_t_read_some `{Eq T} :
+  forall (m : memory T) t t' (NEQ : t <> t'),
+  read (remove_t m t) t' = read m t'.
+Proof.
+  induction m; ii; ss; repeat des_goal; repeat des_hyp;
+  try rewrite eqb_eq in *; clarify; eauto.
+Qed.
+
+Lemma reach_m_step_dec `{Eq T} :
+  forall m acc,
   match reach_m_step acc m with
-  | (_, m') => List.length m' <= List.length m
+  | (_, m') => length m' <= length m
+  end.
+Proof.
+  induction m; ii; ss;
+  repeat des_goal; repeat des_hyp; clarify; ss.
+  - pose proof (remove_t_dec m t). nia.
+  - specialize (IHm acc). repeat des_hyp; clarify. nia.
+Qed.
+
+Lemma areach_m_step_dec `{Eq T} :
+  forall (m : memory T) acc,
+  match areach_m_step acc m with
+  | (_, m') => length m' <= length m
   end.
 Proof.
   induction m; intros; simpl; eauto;
   repeat des_goal; repeat des_hyp; clarify; simpl.
-  - pose proof (remove_t_dec_len m t). nia.
+  - specialize (IHm acc). 
+    repeat des_hyp; clarify. auto.
   - specialize (IHm acc).
     repeat des_hyp; clarify. nia.
 Qed.
+
+Lemma reach_m_step_same `{Eq T} :
+  forall m acc,
+  match reach_m_step acc m with
+  | (acc', m') =>
+    if length m =? length m' then
+      acc = acc' /\ m = m'
+    else True
+  end.
+Proof.
+  induction m; ii; ss; repeat des_goal; repeat des_hyp; des; clarify;
+  rewrite Nat.eqb_eq in *; clarify.
+  - pose proof (reach_m_step_dec m acc).
+    pose proof (remove_t_dec m t).
+    repeat des_hyp; clarify. nia.
+  - ss.
+    assert (length m = length l2) as RR. nia.
+    rewrite <- Nat.eqb_eq in RR.
+    specialize (IHm acc).
+    repeat des_hyp; clarify; des; clarify.
+Qed.
+
+Fixpoint areach_m_aux `{Eq T} acc (m : memory T) fuel :=
+  match areach_m_step acc m with
+  | (acc, m') =>
+    if Nat.eqb (List.length m) (List.length m') then
+      Some acc
+    else match fuel with
+    | 0 => None
+    | S fuel => areach_m_aux acc m' fuel
+    end
+  end.
+
+Definition reach_m `{Eq T} init (m : memory T) :=
+  reach_m_aux init m (List.length m).
+
+Definition areach_m `{Eq T} init (m : memory T) :=
+  areach_m_aux init m (List.length m).
 
 Lemma reach_m_aux_some `{Eq T} :
   forall fuel m init (GE : (List.length m) <= fuel),
@@ -457,12 +739,31 @@ Proof.
   assert (List.length m <= fuel). { nia. }
   repeat des_goal; repeat des_hyp; clarify; eauto; apply IHfuel;
   match goal with
-  | _ => pose proof (remove_t_dec_len m t); nia
-  | _ => idtac
+  | _ : context [remove_t ?m ?t] |- _ =>
+    pose proof (remove_t_dec m t);
+    repeat des_hyp; ss; clarify; try nia
+  | _ : context [reach_m_step ?init ?m] |- _ =>
+    pose proof (reach_m_step_dec m init);
+    repeat des_hyp; ss; clarify
   end.
-  - pose proof (reach_m_step_dec_len m init).
-    repeat des_hyp; ss; clarify.
-    rewrite Nat.eqb_neq in *. nia.
+  - rewrite Nat.eqb_neq in *. nia.
+Qed.
+
+Lemma areach_m_aux_some `{Eq T} :
+  forall fuel m init (GE : (List.length m) <= fuel),
+    exists reached, areach_m_aux init m fuel = Some reached.
+Proof.
+  induction fuel; intros; destruct m; simpl in *; eauto;
+  try (inversion GE; fail).
+  assert (List.length m <= fuel). { nia. }
+  repeat des_goal; repeat des_hyp; clarify; eauto; apply IHfuel;
+  match goal with
+  | _ => rw; nia
+  | _ =>
+    pose proof (areach_m_step_dec m init);
+    repeat des_hyp; ss; clarify;
+    rewrite Nat.eqb_neq in *; nia
+  end.
 Qed.
 
 Lemma relax_fuel `{Eq T} :
@@ -480,19 +781,1104 @@ Proof.
     apply IHfuel with (fuel' := fuel); eauto.
 Qed.
 
+Lemma arelax_fuel `{Eq T} :
+  forall fuel fuel' (LE : fuel' <= fuel) init m reached
+    (EV : areach_m_aux init m fuel' = Some reached),
+  areach_m_aux init m fuel = Some reached.
+Proof.
+  induction fuel;
+  ii; inv LE; ss; repeat des_goal; repeat des_hyp; clarify;
+  apply IHfuel in EV; eauto.
+  - rewrite <- EV. symmetry.
+    eapply IHfuel; eauto.
+    destruct fuel'; ss; repeat rw; eauto.
+  - destruct fuel; ss; repeat des_hyp; clarify.
+    apply IHfuel with (fuel' := fuel); eauto.
+Qed.
+
 Lemma reach_m_some `{Eq T} :
   forall m init, exists reached, reach_m init m = Some reached.
 Proof.
   intros. unfold reach_m. apply reach_m_aux_some. eauto.
 Qed.
 
-Inductive Mpath {T} : path T -> Prop :=
-  | Mnil
-    : Mpath Pnil
-  | Mcons
-    (p : path T) (M : ID) (C : dy_ctx T) (Mp : Mpath p)
-    : Mpath (p +++ (PM M (Ctx C) Pnil))
-.
+Lemma areach_m_some `{Eq T} :
+  forall m init, exists reached, areach_m init m = Some reached.
+Proof.
+  intros. unfold areach_m. apply areach_m_aux_some. eauto.
+Qed.
+
+Definition reach `{Eq T} (n : node T) (m : memory T) :=
+  match n with
+  | Ctx C => reach_m (reach_C [] [] C C) m
+  | Ptr t =>
+    let init := match read m t with
+    | Some (Closure x e C) => 
+      (Ev (Ptr t) (v_fn x e) (Ctx C)) ::
+      reach_C [] [] C C
+    | None => []
+    end in
+    reach_m init (remove_t m t)
+  end.
+
+Fixpoint flatten {T} (ll : list (list T)) :=
+  match ll with
+  | [] => []
+  | l :: tll => l ++ flatten tll
+  end.
+
+Definition areach `{Eq T} (n : node T) (m : memory T) :=
+  match n with
+  | Ctx C => areach_m (reach_C [] [] C C) m
+  | Ptr t => 
+    let init := flatten (map (fun v => match v with
+    | Closure x e C => 
+      (Ev (Ptr t) (v_fn x e) (Ctx C)) ::
+      reach_C [] [] C C
+    end) (aread m t)) in
+    areach_m init (remove_t m t)
+  end.
+
+Fixpoint memify `{Eq T} (edges : list (edge T)) : memory T :=
+  match edges with
+  | [] => []
+  | Ev (Ptr t) (v_fn x e) (Ctx C) :: tl =>
+    (t, Closure x e C) :: memify tl
+  | _ :: tl => memify tl
+  end.
+
+Lemma app_memify `{Eq T} :
+  forall l1 l2,
+    memify (l1 ++ l2) = memify l1 ++ memify l2.
+Proof.
+  induction l1; ii; ss;
+  repeat des_goal; repeat des_hyp; clarify.
+  rw. reflexivity.
+Qed.
+
+Lemma valid_edge_C `{Eq T} :
+  forall e m C (LEFT : Ctx C = lvertex e),
+  valid_edge m e <-> valid_edge [] e.
+Proof.
+  ii. destruct e; ss; repeat des_goal; repeat des_hyp; clarify.
+Qed.
+
+Definition reach_C_pre `{Eq T} seenx seenM (Cout Cin : dy_ctx T) :=
+  (forall x (NIN : ~ In x seenx),
+    match addr_x Cout x, addr_x Cin x with
+    | Some tx, Some tx' => tx = tx'
+    | None, None => True
+    | _, _ => False
+    end) /\
+  (forall M (NIN : ~ In M seenM),
+    match ctx_M Cout M, ctx_M Cin M with
+    | Some CM, Some CM' => CM = CM'
+    | None, None => True
+    | _, _ => False
+    end).
+
+Definition reach_C_post `{Eq T} seenx seenM Cout res :=
+  (forall x (NIN : ~ In x seenx),
+  match addr_x Cout x with
+  | Some t => In (Ex (Ctx Cout) x (Ptr t)) res
+  | None => True
+  end) /\
+  (forall M (NIN : ~ In M seenM),
+  match ctx_M Cout M with
+  | Some CM => In (EM (Ctx Cout) M (Ctx CM)) res
+  | None => True
+  end) /\
+  (forall C e e'
+    (IN : In e res)
+    (RIGHT : Ctx C = rvertex e)
+    (LEFT : Ctx C = lvertex e')
+    (VAL : valid_edge [] e'),
+    In e' res) /\
+  (forall e (IN : In e res),
+    valid_edge [] e) /\
+  (forall e C
+    (IN : In e res) 
+    (LEFT : Ctx C = lvertex e),
+    C = Cout \/
+    exists e', Ctx C = rvertex e' /\ In e' res).
+
+Lemma reach_C_pre_post `{Eq T} :
+  forall Cin Cout seenx seenM
+    (INV : reach_C_pre seenx seenM Cout Cin),
+  reach_C_post seenx seenM Cout (reach_C seenx seenM Cout Cin).
+Proof.
+  induction Cin; ii; ss;
+  unfold reach_C_pre in *;
+  unfold reach_C_post in *;
+  des;
+  repeat match goal with
+  | |- _ /\ _ => split
+  end; ii; ss;
+  repeat des_goal; repeat des_hyp; clarify.
+  - exploit INV; eauto. rw. eauto.
+  - exploit INV0; eauto. rw. eauto.
+  - rewrite Inb_eq in *.
+    exploit INV; eauto. rw.
+    ii; repeat des_hyp; clarify.
+    rewrite eqb_ID_eq in *; clarify.
+    exploit (IHCin Cout seenx seenM).
+    split; eauto.
+    ii. exploit (INV x1); eauto.
+    ii; repeat des_hyp; clarify.
+    rewrite eqb_ID_eq in *. clarify.
+    rw. eauto. rw. eauto.
+    ii. des.
+    specialize (x2 x0 NIN).
+    repeat des_hyp; clarify.
+  - rewrite Inb_neq in *.
+    specialize (INV x0 NIN) as HINT.
+    rewrite GDES in *.
+    repeat des_hyp; clarify.
+    rewrite eqb_ID_eq in *; clarify; eauto.
+    right.
+    exploit (IHCin Cout (x :: seenx) seenM).
+    split; eauto.
+    ii. exploit (INV x1).
+    red; ii; ss; eauto.
+    ii. repeat des_hyp; clarify.
+    rewrite eqb_ID_eq in *. ss. clarify. contradict.
+    rw. eauto. rw. eauto.
+    ii. des. exploit (x2 x0).
+    red; ii; ss; des; clarify.
+    rewrite eqb_ID_neq in *. eauto.
+    ii. repeat des_hyp; clarify.
+  - rewrite Inb_eq in *.
+    exploit (IHCin Cout seenx seenM).
+    split; eauto.
+    ii. exploit INV; eauto.
+    ii; repeat des_hyp; clarify.
+    rewrite eqb_ID_eq in *. clarify.
+    rw. eauto. rw. eauto.
+    ii; des.
+    specialize (x0 M NIN).
+    rewrite GDES in *. eauto.
+  - right. rewrite Inb_neq in *.
+    exploit (IHCin Cout (x :: seenx) seenM).
+    split; eauto.
+    ii. exploit (INV x0).
+    red; ii; ss; eauto.
+    ii. repeat des_hyp; clarify.
+    rewrite eqb_ID_eq in *. clarify. ss. contradict.
+    rw. eauto. rw. eauto.
+    ii. des. exploit (x0 M); eauto.
+    rw. eauto.
+  - rewrite Inb_eq in *.
+    specialize (IHCin Cout seenx seenM).
+    exploit IHCin; eauto.
+    split; eauto.
+    ii. exploit INV; eauto.
+    ii; repeat des_hyp; clarify.
+    rewrite eqb_ID_eq in *; clarify.
+    rw. eauto. rw. eauto.
+    ii; des. eauto.
+  - ss. des; clarify.
+    rewrite Inb_neq in *.
+    exploit (IHCin Cout (x :: seenx) seenM).
+    split; eauto.
+    ii. exploit (INV x0); eauto.
+    red; ii. apply NIN; ss; eauto.
+    ii. repeat des_hyp; clarify.
+    rewrite eqb_ID_eq in *; clarify.
+    ss; contradict.
+    rw. eauto. rw. eauto.
+    ii. des. eauto.
+  - rewrite Inb_eq in *.
+    exploit (IHCin Cout seenx seenM).
+    split; eauto.
+    ii. exploit INV; eauto.
+    ii; repeat des_hyp; clarify.
+    rewrite eqb_ID_eq in *; clarify.
+    rw. eauto. rw. eauto.
+    ii. des. eauto.
+  - rewrite Inb_neq in *.
+    des; clarify; ss.
+    + exploit INV; eauto.
+      ii. repeat des_hyp; try rewrite eqb_ID_neq in *; clarify.
+    + exploit (IHCin Cout (x :: seenx) seenM).
+      split; eauto.
+      ii. exploit (INV x0); eauto.
+      ii; ss; eauto.
+      ii. repeat des_hyp; clarify.
+      rewrite eqb_ID_eq in *. clarify. ss; contradict.
+      rw. eauto. rw. eauto.
+      ii. des. eauto.
+  - rewrite Inb_eq in *.
+    exploit (IHCin Cout seenx seenM); eauto.
+    split; eauto.
+    ii. exploit (INV x0); eauto.
+    ii; repeat des_hyp; clarify.
+    rewrite eqb_ID_eq in *; clarify.
+    rw. eauto. rw. eauto.
+    ii. des. eauto.
+  - rewrite Inb_neq in *.
+    ss; des; clarify; ss; clarify; eauto.
+    exploit (IHCin Cout (x :: seenx) seenM); eauto.
+    split; eauto.
+    ii. exploit (INV x0).
+    red; ii; ss; eauto.
+    ii; repeat des_hyp; clarify.
+    rewrite eqb_ID_eq in *; clarify. ss; contradict.
+    rw. eauto. rw. eauto.
+    ii. des. exploit x4; eauto.
+    ii. des; clarify; eauto.
+  - rewrite Inb_eq in *.
+    exploit (IHCin2 Cout seenx seenM).
+    split; eauto.
+    ii. exploit INV0; eauto.
+    ii; repeat des_hyp; clarify.
+    rewrite eqb_ID_eq in *; clarify.
+    rw. eauto. rw. eauto.
+    ii. des. exploit x1; eauto. rw. eauto.
+  - rewrite Inb_neq in *.
+    rewrite in_app_iff. right. right.
+    exploit (IHCin2 Cout seenx (M :: seenM)).
+    split; eauto.
+    ii. exploit (INV0 M0); eauto.
+    red; ii. ss; eauto.
+    ii; repeat des_hyp; clarify.
+    rewrite eqb_ID_eq in *; ss. contradict.
+    rw. eauto. rw. eauto.
+    ii. des.
+    exploit x1; eauto. rw. eauto.
+  - rewrite Inb_eq in *.
+    exploit (IHCin2 Cout seenx seenM).
+    split; eauto.
+    ii. exploit (INV0 M1); eauto.
+    ii; repeat des_hyp; clarify.
+    rewrite eqb_ID_eq in *; ss; clarify.
+    rw. eauto. rw. eauto.
+    ii. des. exploit (x1 M0); eauto.
+    rw. eauto.
+  - rewrite Inb_neq in *.
+    specialize (INV0 M0 NIN) as HINT.
+    rewrite GDES in HINT.
+    repeat des_hyp; clarify.
+    rewrite eqb_ID_eq in *; clarify.
+    rewrite in_app_iff. right. left. eauto.
+    rewrite eqb_ID_neq in *.
+    exploit (IHCin2 Cout seenx (M :: seenM)).
+    split; eauto.
+    ii. exploit (INV0 M1); eauto.
+    red; ii; ss; eauto.
+    ii; repeat des_hyp; clarify.
+    rewrite eqb_ID_eq in *; ss; clarify. contradict.
+    rw. eauto. rw. eauto.
+    ii. des. exploit (x1 M0); eauto.
+    red; ii; ss; des; clarify.
+    ii; repeat des_hyp; clarify.
+    rewrite in_app_iff. right. right. assumption.
+  - rewrite Inb_eq in *.
+    exploit (IHCin2 Cout seenx seenM).
+    split; eauto.
+    ii. exploit INV0; eauto.
+    ii; repeat des_hyp; clarify.
+    rewrite eqb_ID_eq in *; clarify.
+    rw. eauto. rw. eauto.
+    ii. des. eauto.
+  - rewrite Inb_neq in *.
+    rewrite in_app_iff in *. ss. des; clarify; ss; clarify.
+    + left. specialize (IHCin1 Cin1 [] []).
+      exploit IHCin1.
+      split; ii; ss; repeat des_goal; repeat des_hyp; clarify.
+      ii; des. eauto.
+    + left. specialize (IHCin1 Cin1 [] []).
+      destruct e'; ss; repeat des_hyp; clarify;
+      exploit IHCin1;
+      match goal with
+      | |- _ /\ _ =>
+        split; ii; ss; repeat des_goal; repeat des_hyp; clarify
+      | _ => ii; des
+      end.
+      exploit x1; eauto. rw. eauto.
+      exploit x1; eauto. rw. eauto.
+    + right. right.
+      specialize (IHCin2 Cout seenx (M :: seenM)).
+      exploit IHCin2.
+      split; eauto.
+      ii. exploit (INV0 M0); eauto.
+      red; ii; ss; eauto.
+      ii; repeat des_hyp; clarify.
+      rewrite eqb_ID_eq in *; ss; clarify. contradict.
+      rw. eauto. rw. eauto.
+      ii. des. eauto.
+  - rewrite Inb_eq in *.
+    exploit (IHCin2 Cout seenx seenM).
+    split; eauto.
+    ii. exploit INV0; eauto.
+    ii; repeat des_hyp; clarify.
+    rewrite eqb_ID_eq in *; clarify.
+    rw. eauto. rw. eauto.
+    ii. des. eauto.
+  - rewrite Inb_neq in *.
+    rewrite in_app_iff in *. ss.
+    des; clarify.
+    + exploit (IHCin1 Cin1 [] []).
+      split; ii; ss;
+      repeat des_goal; repeat des_hyp; clarify.
+      ii; des. eauto.
+    + exploit INV0; eauto.
+      ii. repeat des_hyp; clarify.
+      ss. rw. eauto.
+      rewrite eqb_ID_neq in *. contradict.
+      rewrite eqb_ID_neq in *. contradict.
+    + exploit (IHCin2 Cout seenx (M :: seenM)).
+      split; eauto.
+      ii. exploit (INV0 M0); eauto.
+      red; ii; ss; eauto.
+      ii; repeat des_hyp; clarify.
+      rewrite eqb_ID_eq in *; ss; clarify. contradict.
+      rw. eauto. rw. eauto.
+      ii. des. eauto.
+  - rewrite Inb_eq in *.
+    exploit (IHCin2 Cout seenx seenM).
+    split; eauto.
+    ii. exploit (INV0 M0); eauto.
+    ii. repeat des_hyp; clarify.
+    rewrite eqb_ID_eq in *; clarify.
+    rw. eauto. rw. eauto.
+    ii. des. eauto.
+  - rewrite Inb_neq in *.
+    rewrite in_app_iff in *. ss.
+    des; clarify.
+    + exploit (IHCin1 Cin1 [] []).
+      split; ii; repeat des_goal; repeat des_hyp; clarify.
+      ii. des.
+      exploit (INV0 M); eauto.
+      ii. repeat des_hyp; clarify;
+      try rewrite eqb_ID_neq in *; try contradict.
+      exploit x4; eauto.
+      ii. des; clarify.
+      * right. exists (EM (Ctx Cout) M (Ctx d0)).
+        split; ss. rewrite in_app_iff; ss. eauto.
+      * right. exists e'.
+        rewrite in_app_iff; ss; eauto.
+    + ss; clarify; eauto.
+    + exploit (IHCin2 Cout seenx (M :: seenM)).
+      split; eauto.
+      ii. exploit (INV0 M0); eauto.
+      red; ii; ss; eauto.
+      ii; repeat des_hyp; clarify.
+      rewrite eqb_ID_eq in *; ss; clarify. contradict.
+      rw. eauto. rw. eauto.
+      ii. des.
+      exploit x4; eauto. ii; des; clarify; eauto.
+      right. exists e'. rewrite in_app_iff; ss; eauto.
+Qed.
+
+Lemma reach_C_no_t `{Eq T} :
+  forall Cin Cout seenx seenM t,
+  InL (Ptr t) (reach_C seenx seenM Cout Cin) = false.
+Proof.
+  induction Cin; ii; ss; repeat des_goal; repeat des_hyp; clarify.
+  match goal with
+  | |- InL ?a ?b = _ =>
+    destruct (InL a b) eqn:CASE; try reflexivity
+  end.
+  rewrite InL_app_iff in CASE; ss; des.
+  rewrite IHCin1 in *. clarify.
+  rewrite IHCin2 in *. clarify.
+Qed.
+
+Definition reach_C_spec `{Eq T} C res :=
+  (forall e (INe : In e res),
+    valid_edge [] e) /\
+  (forall e (LEFT : Ctx C = lvertex e)
+    (VAL : valid_edge [] e),
+    In e res) /\
+  (forall e e' C (INe : In e res)
+    (INC : Ctx C = lvertex e \/ Ctx C = rvertex e)
+    (LEFT : Ctx C = lvertex e')
+    (VAL : valid_edge [] e'),
+    In e' res) /\
+  (forall e t (LEFT : Ptr t = lvertex e),
+    ~ In e res).
+
+Lemma reach_C_spec_true `{Eq T} :
+  forall C, reach_C_spec C (reach_C [] [] C C).
+Proof.
+  intros.
+  pose proof (reach_C_pre_post C C [] []) as HINT.
+  exploit HINT.
+  unfold reach_C_pre. split; ii; repeat des_goal; clarify.
+  clear HINT. intros HINT.
+  unfold reach_C_post in HINT. des.
+  repeat split; eauto.
+  - ii. destruct e; ss; repeat des_hyp; clarify.
+    exploit HINT; eauto. rw. eauto.
+    exploit HINT0; eauto. rw. eauto.
+  - ii; des.
+    exploit HINT3; eauto. ii. des; clarify.
+    destruct e'; ss; repeat des_hyp; clarify.
+    { exploit HINT; eauto. rw. eauto. }
+    { exploit HINT0; eauto. rw. eauto. }
+    exploit HINT1; eauto.
+    exploit HINT1; eauto.
+  - red; ii.
+    pose proof (reach_C_no_t C C [] [] t).
+    match goal with
+    | _ : InL ?a ?b = false |- _ =>
+      let HINT := fresh "HINT" in
+      assert (InL a b <> true) as HINT;
+      first [apply HINT | refl_bool; ii; clarify]
+    end.
+    rewrite InL_In. exists e. eauto.
+Qed.
+
+Lemma reach_C_path_left `{Eq T} :
+  forall Cin Cout seenx seenM e
+    (PRE : reach_C_pre seenx seenM Cout Cin)
+    (IN : In e (reach_C seenx seenM Cout Cin)),
+    reachable (Ctx Cout) [] e.
+Proof.
+  induction Cin; ii; ss;
+  repeat des_hyp; clarify.
+  - rewrite Inb_eq in *.
+    unfold reach_C_pre in PRE.
+    des; ss.
+    eapply IHCin; eauto.
+    split; eauto.
+    ii. exploit (PRE x0); eauto.
+    ii. repeat des_hyp; clarify.
+    rewrite eqb_ID_eq in *; clarify.
+    rw. eauto. rw. eauto.
+  - rewrite Inb_neq in *.
+    unfold reach_C_pre in PRE.
+    des; clarify.
+    specialize (PRE x HDES).
+    repeat des_hyp; clarify.
+    exists (Px x (Ptr t0) Pnil).
+    ss. rw. eauto.
+    rewrite eqb_ID_neq in *. contradict.
+    rewrite eqb_ID_neq in *. contradict.
+    eapply IHCin; eauto.
+    split; eauto.
+    ii. exploit (PRE x0); eauto.
+    ss. red; ii; eauto.
+    ii. repeat des_hyp; clarify.
+    rewrite eqb_ID_eq in *; clarify; ss; contradict.
+    rw. eauto. rw. eauto.
+  - rewrite Inb_eq in *.
+    unfold reach_C_pre in PRE.
+    des; ss.
+    eapply IHCin2; eauto.
+    split; eauto.
+    ii. exploit (PRE0 M0); eauto.
+    ii. repeat des_hyp; clarify.
+    rewrite eqb_ID_eq in *; clarify.
+    rw. eauto. rw. eauto.
+  - rewrite in_app_iff in *.
+    rewrite Inb_neq in *.
+    ss. des; clarify.
+    + exploit (IHCin1 Cin1 [] [] e); eauto.
+      red; ii. split; ii; repeat des_goal; clarify.
+      ii. unfold reachable in *; des.
+      exists (PM M (Ctx Cin1) p).
+      split; ss; eauto.
+      unfold reach_C_pre in PRE. des.
+      exploit (PRE0 M); eauto.
+      ii. repeat des_hyp; clarify;
+      rewrite eqb_ID_neq in *; contradict.
+    + exists (PM M (Ctx Cin1) Pnil).
+      split; ss; eauto.
+      unfold reach_C_pre in PRE. des.
+      exploit (PRE0 M); eauto.
+      ii. repeat des_hyp; clarify;
+      rewrite eqb_ID_neq in *; clarify.
+    + eapply IHCin2; eauto.
+      unfold reach_C_pre in *; ss; des.
+      split; eauto.
+      ii. exploit (PRE0 M0).
+      red; ii; eauto.
+      ii. repeat des_hyp; clarify.
+      rewrite eqb_ID_eq in *; clarify. contradict.
+      rw. eauto. rw. eauto.
+Qed.
+
+Lemma reach_C_eq_def `{Eq T} :
+  forall C e,
+  reachable (Ctx C) [] e <->
+  In e (reach_C [] [] C C).
+Proof.
+  ii. split; intros REACH.
+  pose proof (reach_C_spec_true C) as SPEC.
+  unfold reach_C_spec in SPEC. des.
+  unfold reachable in *. des.
+  remember (reach_C [] [] C C) as l.
+  clear Heql.
+  ginduction p; ii; ss;
+  repeat des_hyp; clarify; des; clarify.
+  - eapply SPEC0; ss; try rw; eauto.
+  - destruct p; ss; des; clarify;
+    repeat des_hyp; des; clarify.
+  - eapply SPEC0; ss; try rw; eauto.
+  - eapply IHp; eauto. ii.
+    exploit (SPEC1 (EM (Ctx C) M (Ctx d))); ss; eauto.
+    eapply SPEC0; ss; try rw; eauto.
+  - eapply reach_C_path_left; eauto.
+    split; ii; repeat des_goal; eauto.
+Qed.
+
+Lemma no_t_memify_empty `{Eq T} :
+  forall l (NO : forall t, InL (Ptr t) l = false),
+    memify l = [].
+Proof.
+  induction l; ii; ss; repeat des_goal; repeat des_hyp;
+  ss; clarify; eauto;
+  match goal with
+  | NO : forall t, eqb t ?t' || _ = false |- _ =>
+    solve [specialize (NO t'); rewrite t_refl in NO; ss]
+  end.
+Qed.
+
+Lemma reach_C_memify_empty `{Eq T} :
+  forall seenx seenM Cout Cin,
+    memify (reach_C seenx seenM Cout Cin) = [].
+Proof.
+  intros. apply no_t_memify_empty.
+  apply reach_C_no_t.
+Qed.
+
+Definition step_pre `{Eq T}
+  (n : node T) (m : memory T) (E : list (edge T)) :=
+  (forall e,
+    In e E <-> 
+    (valid_edge (memify E) e /\
+      (n = lvertex e \/
+      exists e',
+        In e' E /\
+        rvertex e' = lvertex e))) /\
+  (forall t (IN : InL (Ptr t) E = true),
+    None = read m t).
+
+Lemma reach_C_step_pre `{Eq T} :
+  forall C m, step_pre (Ctx C) m (reach_C [] [] C C).
+Proof.
+  intros. unfold step_pre. split.
+  - intros.
+    rewrite reach_C_memify_empty.
+    rewrite <- reach_C_eq_def.
+    split; ii.
+    rewrite reachable_eq_def in *; des; eauto.
+    rewrite reach_C_eq_def in *. eauto.
+    rewrite reachable_eq_def in *; des; eauto.
+    rewrite <- reach_C_eq_def in *. eauto.
+  - ii. rewrite reach_C_no_t in *. clarify.
+Qed.
+
+Lemma read_memify_In `{Eq T} :
+  forall E (PRE : forall e, In e E -> valid_edge (memify E) e)
+    t x e C,
+    Some (Closure x e C) = read (memify E) t <->
+    In (Ev (Ptr t) (v_fn x e) (Ctx C)) E.
+Proof.
+  ii. split; intros IN.
+  - clear PRE.
+    induction E; ii; ss;
+    repeat des_goal; repeat des_hyp; clarify; 
+    ss; clarify; eauto.
+    rewrite eqb_eq in *; clarify. eauto.
+  - assert (forall x' e' C', 
+      In (Ev (Ptr t) (v_fn x' e') (Ctx C')) E ->
+      x' = x /\ e' = e /\ C' = C).
+    intros x' e' C' IN'.
+    apply PRE in IN, IN'. ss.
+    des. repeat des_hyp; des; clarify.
+    rewrite <- IN in *. clarify.
+    clear PRE.
+    ginduction E; ii; ss;
+    repeat des_goal; repeat des_hyp; clarify;
+    des; clarify; try solve [apply IHE; eauto].
+    rewrite eqb_eq in *. clarify.
+    exploit (H0 x0 e0 C0); eauto. ii; des; clarify.
+    rewrite t_refl in *. clarify.
+Qed.
+
+Lemma step_pre_post_true `{Eq T} :
+  forall n m acc (INV : step_pre n m acc),
+  let (acc', m') := reach_m_step acc m in
+  step_pre n m' acc' /\
+  same (memify acc ++ m) (memify acc' ++ m') /\
+  (exists acc'',
+    acc' = acc'' ++ acc /\
+    (forall t
+      (RIGHT : InR (Ptr t) acc = true)
+      (READ : None <> read m t),
+      exists t',
+        InL (Ptr t') acc'' = true /\
+        None <> read m t') /\
+    (forall t
+      (RIGHT : InR (Ptr t) acc = false),
+      InL (Ptr t) acc'' = false)).
+Proof.
+  induction m; ii;
+  repeat des_goal; repeat des_hyp; ss; clarify.
+  split; eauto.
+  split; ii; eauto.
+  exists []. split. reflexivity.
+  split. ii. contradict. ii; ss.
+  unfold step_pre in INV. des.
+  assert (step_pre n m acc) as PRE.
+  {
+    split; eauto. ii.
+    exploit INV0; eauto; ii; ss; repeat des_hyp; clarify.
+  }
+  repeat des_hyp; ss; clarify. (* 2 goals *)
+  - assert (None = read (memify acc) t) as NREAD.
+    {
+      clear IHm INV HDES PRE.
+      assert (InL (Ptr t) acc = false).
+      refl_bool. intros contra.
+      apply INV0 in contra. rewrite t_refl in *. clarify.
+      clear INV0 n m x e0 C.
+      ginduction acc; ii; ss;
+      repeat des_goal; repeat des_hyp; des; clarify; eauto.
+      ss. clarify.
+      rewrite eqb_eq in *. clarify.
+      rewrite eqb_neq in *. contradict.
+    }
+    split. split; ii. (* 3 goals *)
+    + rewrite in_app_iff. rewrite app_memify.
+      rewrite reach_C_memify_empty. simpl.
+      split; intros IN; des. (* 5 goals *)
+      * rewrite <- reach_C_eq_def in IN.
+        rewrite reachable_eq_def in IN. des; clarify.
+        split. destruct e; repeat des_hyp; ss; clarify.
+        right. exists (Ev (Ptr t) (v_fn x e0) (Ctx C)).
+        rewrite in_app_iff. ss. eauto.
+        split.
+        destruct e; ss; repeat des_hyp; des; clarify.
+        right. exists e'. rewrite in_app_iff. split; eauto.
+        left. rewrite <- reach_C_eq_def. eauto.
+      * clarify. ss. rewrite t_refl.
+        split. exists (Closure x e0 C). eauto.
+        right. rewrite InR_In in HDES. des.
+        exists e. rewrite in_app_iff. ss. eauto.
+      * rewrite INV in IN. destruct IN as [VAL LEFT].
+        split.
+        destruct e; ss; repeat des_hyp; clarify.
+        des; repeat des_hyp; des; clarify;
+        exists (Closure x0 e C0); des_goal; eauto;
+        rewrite eqb_eq in *; clarify; rewrite <- VAL in *; clarify.
+        des; eauto. right. exists e'. rewrite in_app_iff; ss; eauto.
+      * destruct n.
+        destruct (eqb t0 t) eqn:CASE;
+        try rewrite eqb_eq in *; clarify;
+        destruct e; ss; repeat des_hyp; clarify;
+        des; des_hyp; des; clarify; eauto.
+        rewrite <- NREAD in *. clarify.
+        rewrite eqb_eq in *; clarify. rewrite t_refl in *. clarify.
+        right. right. rewrite INV.
+        split. ss. exists (Closure x0 e C0). eauto.
+        ss. eauto.
+        right. right. rewrite INV.
+        rewrite valid_edge_C in *; eauto.
+      * rewrite in_app_iff in *. ss; des.
+        (* case 1 *)
+        destruct e; ss; repeat des_hyp; clarify;
+        try (left; rewrite <- reach_C_eq_def in *;
+            rewrite reachable_eq_def; split;
+            solve [ss; rw; reflexivity
+            | right; exists e'; ss]).
+        rewrite eqb_eq in *. clarify.
+        des. clarify. des. clarify. eauto.
+        des. right. right. rewrite INV.
+        des_hyp. des. clarify.
+        assert (In (Ev (Ptr t0) (v_fn x0 e) (Ctx C0)) acc) as HINT.
+        rewrite <- read_memify_In; eauto.
+        ii. rewrite INV in *. des; eauto.
+        rewrite INV in HINT.
+        des; eauto.
+        (* case 2 *)
+        clarify; ss. left.
+        rewrite <- reach_C_eq_def.
+        rewrite valid_edge_C in IN; eauto.
+        rewrite reachable_eq_def. eauto.
+        (* case 3 *)
+        destruct (lvertex e) eqn:CASE.
+        destruct e; ss; repeat des_hyp; clarify.
+        rewrite eqb_eq in *; clarify. des. des_hyp. des. clarify. eauto.
+        right. right. rewrite INV. ss. eauto.
+        rewrite valid_edge_C in IN; eauto.
+        rewrite <- valid_edge_C with (m := memify acc) in IN; eauto.
+        right. right. rewrite INV. split; eauto.
+        right. exists e'. split; eauto. repeat rw. eauto.
+    + rewrite InL_app_iff in *.
+      des. rewrite reach_C_no_t in *. clarify.
+      ss. des_hyp. rewrite eqb_eq in *; clarify.
+      apply remove_t_read.
+      exploit INV0; eauto. des_goal. clarify.
+      rewrite eqb_neq in *.
+      ii. rewrite remove_t_read_some; eauto.
+    + split.
+      * rewrite app_memify. rewrite reach_C_memify_empty. simpl.
+        repeat match goal with
+        | |- context [(?t, ?v) :: ?l] =>
+          lazymatch l with
+          | [] => fail
+          | _ => replace ((t, v) :: l) with ([(t, v)] ++ l) by reflexivity
+          end
+        end.
+        repeat rewrite app_assoc.
+        eapply same_trans.
+        instantiate (1 := (memify acc ++ [(t, Closure x e0 C)]) ++ remove_t m t).
+        repeat rewrite <- app_assoc. apply app_same. ii; ss.
+        ii; ss. des_goal; clarify. rewrite eqb_neq in *.
+        rewrite remove_t_read_some; eauto.
+        apply app_same. apply app_disj_same.
+        ii. ss. des_goal; clarify. rewrite eqb_eq in *. clarify.
+        ii. ss.
+      * exists (reach_C [] [] C C ++ [Ev (Ptr t) (v_fn x e0) (Ctx C)]).
+        split. rewrite <- app_assoc. ss.
+        split. ii. exists t. rewrite t_refl.
+        split; ii; clarify.
+        rewrite InL_In. exists (Ev (Ptr t) (v_fn x e0) (Ctx C)).
+        rewrite in_app_iff. split; ss; eauto.
+        ii. refl_bool. ii.
+        rewrite InL_app_iff in *. des.
+        rewrite reach_C_no_t in *. clarify.
+        ss. des_hyp. rewrite eqb_eq in *. clarify.
+  - exploit IHm; eauto. intros POST.
+    repeat des_hyp; des; clarify.
+    unfold step_pre in POST. des.
+    assert (InL (Ptr t) acc = false) as NIN.
+    refl_bool. ii. exploit INV0; eauto. rewrite t_refl. clarify.
+    assert (InL (Ptr t) acc'' = false) as NIN'. eauto.
+    split; split; try assumption. (* 3 goals *)
+    + ii. exploit POST1; eauto. ii.
+      ss. des_goal; clarify. rewrite eqb_eq in *; clarify.
+      rewrite InL_app_iff in IN. des; clarify.
+    + repeat match goal with
+      | |- context [(?t, ?v) :: ?l] =>
+        lazymatch l with
+        | [] => fail
+        | _ => replace ((t, v) :: l) with ([(t, v)] ++ l) by reflexivity
+        end
+      end.
+      repeat rewrite app_assoc.
+      eapply same_trans.
+      instantiate (1 := ([(t, e)] ++ memify acc) ++ m).
+      apply app_same.
+      apply app_disj_same.
+      ii; ss. des_goal; eauto.
+      rewrite eqb_eq in *. clarify.
+      destruct (read (memify acc) t0) eqn:READ'; clarify.
+      symmetry in READ'.
+      destruct e0. rewrite read_memify_In in *.
+      assert (InL (Ptr t0) acc = true).
+      rewrite InL_In. exists (Ev (Ptr t0) (v_fn x e0) (Ctx C)). ss.
+      clarify.
+      ii. rewrite INV in *. des; eauto.
+      ii; ss.
+      eapply same_trans.
+      instantiate (1 := ([(t, e)] ++ memify (acc'' ++ acc)) ++ l2).
+      repeat rewrite <- app_assoc. ss.
+      solve [ii; ss; des_goal; eauto].
+      apply  app_same.
+      apply app_disj_same.
+      ii; ss. des_hyp; clarify.
+      rewrite eqb_eq in *. clarify.
+      match goal with |- None = ?x => destruct x eqn:CASE end; try reflexivity.
+      symmetry in CASE.
+      destruct e0. rewrite read_memify_In in CASE.
+      rewrite in_app_iff in *. des.
+      assert (InL (Ptr t0) acc'' = true).
+      rewrite InL_In. exists (Ev (Ptr t0) (v_fn x e0) (Ctx C)). ss.
+      clarify.
+      assert (InL (Ptr t0) acc = true).
+      rewrite InL_In. exists (Ev (Ptr t0) (v_fn x e0) (Ctx C)). ss.
+      clarify.
+      ii. rewrite POST in *. des; eauto.
+      ii; ss.
+    + exists acc''. split; eauto.
+      split; ii; eauto.
+      des_hyp; clarify.
+      rewrite eqb_eq in *; clarify.
+      exploit POST2; eauto. ii. des.
+      exists t'. split; eauto.
+      des_goal; clarify.
+Qed.
+
+Lemma step_spec_left `{Eq T} :
+  forall E n
+    (PRE : forall e, (valid_edge (memify E) e /\
+      (n = lvertex e \/
+      exists e',
+        In e' E /\
+        rvertex e' = lvertex e)) -> In e E)
+    e (REACH : reachable n (memify E) e),
+  In e E.
+Proof.
+  ii.
+  unfold reachable in REACH. des.
+  ginduction p; ii; ss; repeat des_hyp; clarify;
+  des; clarify; try des_hyp; des; clarify.
+  - apply PRE. ss. rw. eauto.
+  - eapply IHp with (n := (Ptr t0)); eauto.
+    ii. apply PRE. split; des; eauto.
+    right. exists (Ex (Ctx C) x (Ptr t0)).
+    split; ss; eauto. apply PRE. ss. rw. eauto.
+  - apply PRE. ss. rw. eauto.
+  - eapply IHp with (n := (Ctx d)); eauto.
+    ii. apply PRE. split; des; eauto.
+    right. exists (EM (Ctx C0) M (Ctx d)).
+    split; ss; eauto. apply PRE. ss. rw. eauto.
+  - apply PRE. ss. split; eauto.
+    exists (Closure x e C0); ss.
+  - eapply IHp with (n := (Ctx C0)); eauto.
+    ii. apply PRE. split; des; eauto.
+    right. exists (Ev (Ptr t) (v_fn x e0) (Ctx C0)).
+    split; ss; eauto. apply PRE. ss. split; eauto.
+    exists (Closure x e0 C0); ss.
+Qed.
+
+Lemma vpath_less_then_vpath_more `{Eq T} :
+  forall a b p n (VAL : valid_path n a p),
+  valid_path n (a ++ b) p.
+Proof.
+  ii.
+  ginduction p; ii; ss;
+  repeat des_hyp; des; clarify; eauto.
+  des_hyp; des; clarify.
+  exists (Closure x e C0).
+  rewrite read_top. rewrite <- VAL. eauto.
+Qed.
+
+Lemma vedge_less_then_vedge_more `{Eq T} :
+  forall a b e (VAL : valid_edge a e),
+  valid_edge (a ++ b) e.
+Proof.
+  ii.
+  destruct e; ss; repeat des_hyp; des; clarify.
+  des_hyp; des; clarify.
+  exists (Closure x e C).
+  rewrite read_top. rewrite <- VAL. eauto.
+Qed.
+
+Lemma paste_vpath `{Eq T} :
+  forall n m e (REACH : reachable n m e) e'
+    (REACH' : reachable (rvertex e) m e'),
+  reachable n m e'.
+Proof.
+  ii. destruct REACH as [p [VAL IN]].
+  ginduction p; ii; ss; repeat des_hyp; des; clarify; ss.
+  - destruct REACH' as [p' [VAL' IN']].
+    exists (Px x (Ptr t0) p').
+    ss. rw. eauto.
+  - exploit IHp; eauto. intros REACH.
+    destruct REACH as [p' [VAL' IN']].
+    exists (Px x (Ptr t0) p').
+    ss. rw. eauto.
+  - destruct REACH' as [p' [VAL' IN']].
+    exists (PM M (Ctx d) p').
+    ss. rw. eauto.
+  - exploit IHp; eauto. intros REACH.
+    destruct REACH as [p' [VAL' IN']].
+    exists (PM M (Ctx d) p').
+    ss. rw. eauto.
+  - des_hyp; des; clarify.
+    destruct REACH' as [p' [VAL' IN']].
+    exists (Pv (v_fn x e) (Ctx C0) p').
+    ss. split; eauto.
+    exists (Closure x e C0). eauto.
+  - des_hyp; des; clarify.
+    exploit IHp; eauto. intros REACH.
+    destruct REACH as [p' [VAL' IN']].
+    exists (Pv (v_fn x e0) (Ctx C0) p').
+    ss. split; eauto.
+    exists (Closure x e0 C0). eauto.
+Qed.
+
+Lemma step_spec_right `{Eq T} :
+  forall m n E
+    (PRE : forall e, In e E -> reachable n (memify E) e)
+    (DISJ : forall t, InL (Ptr t) E = true -> None = read m t),
+    let (E', m') := reach_m_step E m in
+    (forall e (IN : In e E'), reachable n (memify E') e) /\
+    (forall t (LEFT : InL (Ptr t) E' = true), None = read m' t) /\
+    (forall t (LEFT : InL (Ptr t) E' = true /\ InL (Ptr t) E = false),
+      InR (Ptr t) E = true).
+Proof.
+  ii.
+  match goal with
+  | |- match ?E with _ => _ end =>
+    destruct E as [E' m'] eqn:STEP
+  end; ii.
+  ginduction m; ii; ss; clarify; eauto.
+  assert (forall e, In e E' -> valid_edge (memify E') e) as HINT.
+  {
+    ii. exploit PRE; eauto. ii.
+    rewrite reachable_eq_def in *. des; eauto.
+  }
+  repeat split; eauto. ii.
+  {
+    des. rewrite InL_In in LEFT. des.
+    apply PRE in LEFT. rewrite reachable_eq_def in LEFT.
+    destruct LEFT as [VAL ?].
+    destruct e; ss; repeat des_hyp; des; clarify;
+    des_hyp; des; clarify;
+    rewrite read_memify_In in VAL; eauto;
+    assert (InL (Ptr t0) E' = true);
+    try solve [rewrite InL_In; exists (Ev (Ptr t0) (v_fn x e) (Ctx C)); eauto];
+    clarify.
+  }
+  des_hyp.
+  assert (InL (Ptr t) E = false) as DISJ'.
+  { refl_bool. intros contra. apply DISJ in contra. rewrite t_refl in *. clarify. }
+  assert (forall e, In e E -> valid_edge (memify E) e) as HINT.
+  {
+    ii. exploit PRE; eauto. ii.
+    rewrite reachable_eq_def in *. des; eauto.
+  }
+  split.
+  repeat des_hyp; clarify; ii.
+  - rewrite InR_In in *. des. rename IN into IN'.
+    match goal with
+    | H : _ |- _ => 
+      apply PRE in H;
+      unfold reachable in H;
+      destruct H as [p [VAL IN]]
+    end.
+    rewrite app_memify. rewrite reach_C_memify_empty. s.
+    assert (forall p', valid_path n (memify E) p' -> 
+      valid_path n ((t, Closure x e0 C) :: memify E) p').
+    {
+      clear IHm PRE DISJ e1 IN HDES1 e IN'.
+      ii. ginduction p'; ii; ss; repeat des_goal; clarify.
+      des; clarify. split; eauto.
+      des; clarify. split; eauto.
+      rewrite eqb_eq in *. clarify.
+      des. des_hyp. rewrite read_memify_In in *; eauto.
+      des; clarify.
+      assert (InL (Ptr t0) E = true).
+      rewrite InL_In.
+      exists (Ev (Ptr t0) (v_fn x0 e) (Ctx C1)). ss.
+      clarify.
+      des. des_hyp. des. clarify.
+      exists (Closure x0 e C1); eauto.
+    }
+    rewrite in_app_iff in *.
+    ss. des; clarify.
+    + rewrite <- reach_C_eq_def in IN'.
+      eapply paste_vpath. instantiate (1 := e1).
+      exists p. split; eauto.
+      rewrite <- HDES1.
+      match goal with
+      | _ : context [(?t, Closure ?x ?e ?C)] |- _ =>
+        eapply paste_vpath;
+        first [
+          instantiate (1 := (Ev (Ptr t) (v_fn x e) (Ctx C)));
+          exists (Pv (v_fn x e) (Ctx C) Pnil);
+          ss; rewrite t_refl; split; eauto;
+          exists (Closure x e C); eauto |
+          idtac]
+      end.
+      ss. destruct IN' as [p' [VAL' IN']].
+      exists p'. split; eauto.
+      eapply vpath_less_then_vpath_more with (a := []). eauto.
+    + eapply paste_vpath. instantiate (1 := e1). exists p. split; eauto.
+      rewrite <- HDES1.
+      match goal with
+      | _ : context [(?t, Closure ?x ?e ?C)] |- _ =>
+        exists (Pv (v_fn x e) (Ctx C) Pnil);
+        ss; rewrite t_refl; split; eauto;
+        exists (Closure x e C); eauto
+      end.
+    + apply PRE in IN'.
+      destruct IN' as [p' [VAL' IN']].
+      exists p'. split; eauto.
+  - exploit IHm; ii; des; eauto.
+    exploit DISJ; eauto.
+    des_goal; clarify.
+  - repeat des_hyp; clarify. repeat split.
+    + ii. rewrite InL_app_iff in LEFT.
+      des. rewrite reach_C_no_t in LEFT. clarify.
+      ss. des_hyp. rewrite eqb_eq in *; clarify.
+      apply remove_t_read.
+      exploit DISJ; eauto.
+      ii. des_hyp; clarify.
+      rewrite eqb_neq in *.
+      rewrite remove_t_read_some; eauto.
+    + ii. rewrite InL_app_iff in LEFT.
+      des. rewrite reach_C_no_t in LEFT. clarify.
+      ss. des_hyp; clarify. rewrite eqb_eq in *; clarify.
+    + exploit IHm; ii; des; eauto.
+      exploit DISJ; eauto.
+      des_goal; clarify.
+      repeat split; eauto.
+      ii. ss. des_goal; eauto.
+      rewrite eqb_eq in *. clarify.
+      assert (InR (Ptr t0) E = true).
+      eauto. clarify.
+Qed.
+
+Lemma step_spec_lemma `{Eq T} :
+  forall m n E
+    (IN : forall e, In e E <-> reachable n (memify E) e)
+    (DISJ : forall t, InL (Ptr t) E || InR (Ptr t) E = true ->
+      None = read m t)
+    (INn : InL n E || InR n E = true) e,
+    In e E <-> reachable n (memify E ++ m) e.
+Proof.
+  ii. rewrite IN.
+  split; intros REACH;
+  destruct REACH as [p [VAL INV]];
+  exists p; split; try assumption.
+  apply vpath_less_then_vpath_more. eauto.
+  assert (forall e, reachable n (memify E) e -> In e E) as REACH.
+  ii. rewrite IN. eauto.
+  clear IN e INV.
+  ginduction p; ii; ss;
+  repeat des_goal; des; clarify.
+  - exploit (REACH (Ex (Ctx C) x (Ptr t0))).
+    exists (Px x (Ptr t0) Pnil). ss. rw. eauto.
+    ii.
+    assert (InR (Ptr t0) E = true).
+    rewrite InR_In. exists (Ex (Ctx C) x (Ptr t0)). ss.
+    split; eauto. eapply IHp; eauto. rw. des_goal; eauto.
+    intros e' REACH'. apply REACH.
+    eapply paste_vpath.
+    instantiate (1 := Ex (Ctx C) x (Ptr t0)).
+    exists (Px x (Ptr t0) Pnil). ss. rw. eauto.
+    ss.
+  - exploit (REACH (EM (Ctx C0) M (Ctx d))).
+    exists (PM M (Ctx d) Pnil). ss. rw. eauto.
+    ii.
+    assert (InR (Ctx d) E = true).
+    rewrite InR_In. exists (EM (Ctx C0) M (Ctx d)). ss.
+    split; eauto. eapply IHp; eauto. rw. des_goal; eauto.
+    intros e' REACH'. apply REACH.
+    eapply paste_vpath.
+    instantiate (1 := EM (Ctx C0) M (Ctx d)).
+    exists (PM M (Ctx d) Pnil). ss. rw. eauto.
+    ss.
+  - destruct ev; des; clarify.
+    rewrite read_top in *.
+    destruct (read (memify E) t) eqn:READ.
+    + clarify. exists (Closure x e C0).
+      repeat split; eauto.
+      eapply IHp; eauto.
+      assert (InR (Ctx C0) E = true).
+      rewrite InR_In.
+      exists (Ev (Ptr t) (v_fn x e) (Ctx C0)).
+      split; eauto. apply REACH.
+      exists (Pv (v_fn x e) (Ctx C0) Pnil).
+      ss. split; eauto. exists (Closure x e C0); eauto.
+      rw. des_goal; eauto.
+      intros e' REACH'. apply REACH.
+      eapply paste_vpath.
+      instantiate (1 := Ev (Ptr t) (v_fn x e) (Ctx C0)).
+      exists (Pv (v_fn x e) (Ctx C0) Pnil).
+      ss. split; eauto. exists (Closure x e C0); eauto.
+      ss.
+    + assert (None = read m t) as RR.
+      apply DISJ. rw. eauto.
+      rewrite <- RR in *. clarify.
+Qed.
 
 Fixpoint prefixof {T} (p p' : path T) :=
   match p, p' with
@@ -529,42 +1915,53 @@ Proof.
   end.
 Qed.
 
-Lemma asame_aequiv `{Eq T} `{Eq TT} :
-  forall (V : dy_value T) m (V' : dy_value TT) m' m''
-    (EQUIV : <|V m ≃# V' m'|>) (SAME : asame m' m''),
-  <|V m ≃# V' m''|>.
+Lemma iso_comm `{Eq T} `{Eq TT} :
+  forall (C : dy_ctx T) m (C' :dy_ctx TT) m' f f',
+  iso C m C' m' f f' <-> iso C' m' C m f' f.
 Proof.
-  intros. red in EQUIV.
-  destruct EQUIV as [f [f' [EQl EQr]]].
-  unfold asame in SAME.
-  red. exists f. exists f'. split; simpl in *.
-  - intros. specialize (EQl p VALp).
-    split; try apply EQl.
-    destruct EQl as [EQ ELSE].
-    clear ELSE EQr VALp. remember (pmap f p) as p'.
-    clear Heqp' p f f' m V.
-    ginduction p'; intros; simpl in *;
-    repeat des_goal; repeat des_hyp; clarify; eauto.
-    + destruct EQ as [? [ev [IN VALp]]]; subst.
-      split; eauto. exists ev.
-      split. rewrite <- SAME. eauto.
-      eapply IHp'; eauto.
-    + destruct EQ as [? VALp]; subst.
-      split; eauto.
-    + destruct EQ as [? [? VALp]]; subst.
-      repeat split; eauto.
-  - intros. apply EQr.
-    clear EQl EQr f f' V.
-    ginduction p'; intros; simpl in *;
-    repeat des_goal; repeat des_hyp; clarify; eauto.
-    + destruct VALp' as [? [ev [IN ?]]]; subst.
-      split; eauto. exists ev.
-      split. rewrite SAME. eauto.
-      eapply IHp'; eauto.
-    + destruct VALp' as [? ?]; subst.
-      split; eauto.
-    + destruct VALp' as [? [? ?]]; subst.
-      repeat split; eauto.
+  ii; split; ii; unfold iso in *; des;
+  repeat (split; eauto).
+Qed.
+
+Lemma asame_comm `{Eq T} :
+  forall m m',
+  asame m m' <-> asame m' m.
+Proof.
+  intros; unfold asame; split; ii; rw; eauto.
+Qed.
+
+Lemma aiso_comm `{Eq T} `{Eq TT} :
+  forall (C : dy_ctx T) m (C' :dy_ctx TT) m' f f',
+  aiso C m C' m' f f' <-> aiso C' m' C m f' f.
+Proof.
+  ii; split; ii; unfold aiso in *; des;
+  repeat (split; eauto).
+Qed.
+
+Lemma same_valid `{Eq T} :
+  forall p n m m' (SAME : same m m')
+    (VALp : valid_path n m p),
+  valid_path n m' p.
+Proof.
+  ii; unfold same in *;
+  ginduction p; intros; ss;
+  repeat des_goal; repeat des_hyp; clarify;
+  des; try split; eauto.
+  - exists ev. split. rewrite <- SAME. eauto.
+    des_hyp; des; repeat split; eauto.
+Qed.
+
+Lemma asame_avalid `{Eq T} :
+  forall p n m m' (SAME : asame m m')
+    (VALp : avalid_path n m p),
+  avalid_path n m' p.
+Proof.
+  ii; unfold asame in *;
+  ginduction p; intros; ss;
+  repeat des_goal; repeat des_hyp; clarify;
+  des; try split; eauto.
+  - exists ev. split. rewrite <- SAME. eauto.
+    des_hyp; des; repeat split; eauto.
 Qed.
 
 Lemma same_equiv `{Eq T} `{Eq TT} :
@@ -572,37 +1969,50 @@ Lemma same_equiv `{Eq T} `{Eq TT} :
     (EQUIV : <|V m ≃ V' m'|>) (SAME : same m' m''),
   <|V m ≃ V' m''|>.
 Proof.
-  intros. red in EQUIV.
-  destruct EQUIV as [f [f' [EQl EQr]]].
-  unfold same in SAME.
-  red. exists f. exists f'. split; simpl in *.
-  - intros. specialize (EQl p VALp).
-    split; try apply EQl.
-    destruct EQl as [EQ ELSE].
-    clear ELSE EQr VALp. remember (pmap f p) as p'.
-    clear Heqp' p f f' m V.
-    ginduction p'; intros; simpl in *;
-    repeat des_goal; repeat des_hyp; clarify; eauto.
-    + destruct EQ as [? [ev [IN VALp]]]; subst.
-      split; eauto. exists ev.
-      split. rewrite <- SAME. eauto.
-      eapply IHp'; eauto.
-    + destruct EQ as [? VALp]; subst.
-      split; eauto.
-    + destruct EQ as [? [? VALp]]; subst.
-      repeat split; eauto.
-  - intros. apply EQr.
-    clear EQl EQr f f' V.
-    ginduction p'; intros; simpl in *;
-    repeat des_goal; repeat des_hyp; clarify; eauto.
-    + destruct VALp' as [? [ev [IN ?]]]; subst.
-      split; eauto. exists ev.
-      split. rewrite SAME. eauto.
-      eapply IHp'; eauto.
-    + destruct VALp' as [? ?]; subst.
-      split; eauto.
-    + destruct VALp' as [? [? ?]]; subst.
-      repeat split; eauto.
+  intros. red in EQUIV; repeat des_hyp; des; clarify; red;
+  repeat split; try reflexivity; exists f; exists f';
+  unfold iso in *; des;
+  (split; 
+  first [assumption | split];
+  first [assumption | split]); ii;
+  match goal with
+  | H : _ |- context [valid_path (Ctx ?C) m''] =>
+    specialize (H p VALp); des; split; eauto;
+    remember (pmap f p) as p';
+    remember (Ctx C) as n;
+    clear Heqn Heqp' VALp
+  | H : context [valid_path (Ctx ?C) m'] |- _ =>
+    apply H; remember (Ctx C) as n;
+    clear Heqn
+  end; 
+  solve [eapply same_valid; eauto |
+  rewrite same_comm in *; eapply same_valid; eauto].
+Qed.
+
+
+Lemma asame_aequiv `{Eq T} `{Eq TT} :
+  forall (V : dy_value T) m (V' : dy_value TT) m' m''
+    (EQUIV : <|V m ≃# V' m'|>) (SAME : asame m' m''),
+  <|V m ≃# V' m''|>.
+Proof.
+  intros. red in EQUIV; repeat des_hyp; des; clarify; red;
+  repeat split; try reflexivity; exists f; exists f';
+  unfold aiso in *; des;
+  (split; 
+  first [assumption | split];
+  first [assumption | split]); ii;
+  match goal with
+  | H : _ |- context [avalid_path (Ctx ?C) m''] =>
+    specialize (H p VALp); des; split; eauto;
+    remember (pmap f p) as p';
+    remember (Ctx C) as n;
+    clear Heqn Heqp' VALp
+  | H : context [avalid_path (Ctx ?C) m'] |- _ =>
+    apply H; remember (Ctx C) as n;
+    clear Heqn
+  end;
+  solve [eapply asame_avalid; eauto |
+  rewrite asame_comm in *; eapply asame_avalid; eauto].
 Qed.
 
 (* lift unreachable Cs *)
