doc/coq/simple/Bound.v
@@ -1,0 +1,308 @@
+From Simple Require Export Abstract.
+From Simple Require Export Concrete.
+
+Ltac lebt x :=
+  apply leb_trans with (t' := x);
+  try assumption; try apply tick_lt; try apply leb_refl.
+
+Generalizable Variables T aT TT aTT.
+
+Definition time_bound_C `{TotalOrder T} C t :=
+  forall t', supp_C C t' -> leb t' t = true.
+
+Definition time_bound_m `{TotalOrder T} m t :=
+  forall t', supp_m m t' -> leb t' t = true.
+
+Definition time_bound_v `{TotalOrder T} v t :=
+  match v with
+  | Closure _ _ C => time_bound_C C t
+  end.
+
+Definition time_bound_V `{TotalOrder T} V t :=
+  match V with
+  | EVal ev => time_bound_v ev t
+  | MVal mv => time_bound_C mv t
+  end.
+
+Definition time_bound_ρ `{TotalOrder T} (ρ : config T) :=
+  match ρ with
+  | Cf _ C m t =>
+    time_bound_C C t /\ time_bound_m m t
+  | Rs V m t =>
+    time_bound_V V t /\ time_bound_m m t
+  end.
+
+Lemma not_le_lt `{TotalOrder T} :
+  forall (p : T) t,
+    (leb p t = false) <-> (t < p).
+Proof.
+  intros; unfold "<"; red; split; intros NLE;
+  repeat match goal with
+  | H : _ /\ _ |- _ => destruct H
+  | |- context [leb ?p ?t] =>
+    let RR := fresh "RR" in
+    destruct (leb p t) eqn:RR
+  | |- context [eqb ?p ?t] =>
+    let RR := fresh "RR" in
+    destruct (eqb p t) eqn:RR
+  | H : context [leb ?p ?t] |- _ =>
+    match goal with
+    | _ : leb p t = true |- _ => idtac
+    | _ : leb p t = false |- _ => idtac
+    | _ =>
+      let RR := fresh "RR" in
+      destruct (leb p t) eqn:RR
+    end
+  end;
+  try rewrite eqb_eq in *;
+  try rewrite eqb_neq in *; subst;
+  try rewrite leb_refl in *;
+  clarify; exfalso; eauto using leb_sym.
+  pose proof leb_or as contra.
+  specialize (contra p t).
+  rewrite NLE in *. rewrite RR in *. clarify.
+Qed.
+
+Lemma time_bound_or_not `{TotalOrder T} :
+  forall (p : T) t,
+    (p < t) \/ ~(p < t).
+Proof.
+  intros.
+  rewrite <- not_le_lt.
+  destruct (leb t p); eauto.
+Qed.
+
+Lemma time_increase `{time T} :
+  forall e C m t cf' (EVAL : {|(Cf e C m t) ~> cf'|}),
+    match cf' with
+    | Cf _ _ _ t'
+    | Rs _ _ t' => leb t t' = true
+    end.
+Proof.
+  intros.
+  remember (Cf e C m t) as cf. ginduction EVAL;
+  intros; clarify; try apply leb_refl; eauto 2;
+  try (exploit IHEVAL3; eauto 1);
+  try (exploit IHEVAL2; eauto 1);
+  try (exploit IHEVAL1; eauto 1);
+  try (exploit IHEVAL; eauto 1); intros;
+  try lebt t';
+  try lebt t_f;
+  try lebt t_a;
+  match goal with
+  | _ : context [tick ?C ?m ?t ?x ?v] |- _ =>
+    lebt (tick C m t x v)
+  end.
+Qed.
+
+Lemma relax_ctx_bound `{time T} :
+  forall C t1 t2 (BOUND : time_bound_C C t1) (LE : leb t1 t2 = true),
+         time_bound_C C t2.
+Proof.
+  induction C; unfold time_bound_C;
+  intros; ss; des; clarify;
+  match goal with
+  | H : supp_C ?C ?t |- _ =>
+    match goal with
+    | H : context [time_bound_C C _] |- _ => eapply H; eauto
+    end
+  | _ => idtac
+  end; try red; intros; try apply BOUND; eauto.
+  - lebt t1. apply BOUND. left; eauto.
+Qed.
+
+Lemma relax_p_bound `{time T} :
+  forall p t1 t2 (BOUND : p < t1) (LE : leb t1 t2 = true),
+    p < t2.
+Proof.
+  intros. destruct BOUND as [? EQ]. split.
+  - lebt t1.
+  - rewrite eqb_neq in *. red; intros.
+    subst. apply EQ. apply leb_sym; eauto.
+Qed.
+
+Lemma relax_mem_bound `{time T} :
+  forall m t1 t2 (BOUND : time_bound_m m t1) (LE : leb t1 t2 = true),
+         time_bound_m m t2.
+Proof.
+  induction m; unfold time_bound_m;
+  intros; ss; repeat des_hyp; clarify.
+  lebt t1. apply BOUND. eauto.
+Qed.
+
+Lemma time_bound_addr `{time T} :
+  forall C x t (BOUND : time_bound_C C t),
+    match addr_x C x with
+    | None => True
+    | Some addr => leb addr t = true
+    end.
+Proof.
+  induction C; unfold time_bound_C; intros; simpl in *; eauto;
+  repeat des_goal; repeat des_hyp; clarify;
+  match goal with
+  | IH : forall _ t, _ |- _ =>
+    match type of IH with
+    | context [addr_x ?C _] =>
+      match goal with
+      | RR : addr_x C ?x = _ |- _ =>
+        specialize (IH x t);
+        rewrite RR in IH;
+        apply IH; red; intros
+      end
+    end
+  | _ => idtac
+  end; apply BOUND; eauto.
+Qed.
+
+Lemma time_bound_read `{time T} :
+  forall m t addr (BOUND : time_bound_m m t),
+    match read m addr with
+    | None => True
+    | Some v => time_bound_v v t
+    end.
+Proof.
+  induction m; intros; simpl; eauto;
+  repeat des_goal; repeat des_hyp; eauto;
+  try rewrite eqb_eq in *; clarify;
+  match goal with
+  | _ => 
+    unfold time_bound_m in *;
+    unfold time_bound_v;
+    des_goal; red; intros; simpl in *;
+    apply BOUND; eauto; fail
+  | RR : read ?m ?addr = Some ?v |- _ => 
+    specialize (IHm t addr);
+    rewrite RR in IHm;
+    apply IHm; red; intros; apply BOUND; simpl; eauto
+  end.
+Qed.
+
+Lemma time_bound_ctx_M `{time T} :
+  forall C M t (BOUND : time_bound_C C t),
+    match ctx_M C M with
+    | None => True
+    | Some CM => time_bound_C CM t
+    end.
+Proof.
+  induction C; unfold time_bound_C; intros; simpl in *; eauto;
+  repeat des_goal; repeat des_hyp; clarify;
+  match goal with
+  | IH : forall _ t, _ |- _ =>
+    match type of IH with
+    | context [ctx_M ?C _] =>
+      match goal with
+      | RR : ctx_M C ?M = _ |- _ =>
+        specialize (IH M t);
+        rewrite RR in IH;
+        apply IH; red; intros
+      end
+    end
+  | _ => idtac
+  end; try apply BOUND; eauto.
+Qed.
+
+Lemma leb_t_neq_tick `{time T} :
+  forall C m x v (t' t : T) (LE : leb t' t = true),
+  eqb t' (tick C m t x v) = false.
+Proof.
+  intros. refl_bool. intros contra.
+  rewrite eqb_eq in *.
+  assert (t <> tick C m t x v) as NEQ.
+  { rewrite <- eqb_neq. apply tick_lt. }
+  apply NEQ. apply leb_sym. 
+  - apply tick_lt.
+  - subst. eauto.
+Qed.
+
+Lemma time_bound_tick `{time T} :
+  forall C m t x v
+         (BOUNDv : time_bound_v v t)
+         (BOUNDm : time_bound_m m t),
+  time_bound_m ((tick C m t x v) !-> v; m) (tick C m t x v).
+Proof.
+  intros.
+  unfold time_bound_v in *.
+  unfold time_bound_m in *. des_hyp.
+  unfold time_bound_C in *.
+  ii; ss; des; clarify;
+  match goal with
+  | |- leb ?t ?t = true => apply leb_refl
+  | H : supp_C ?C _, 
+    BD : forall _, supp_C ?C _ -> _
+    |- leb _ (tick _ _ ?t _ _) = true  =>
+    apply BD in H; lebt t
+  | H : supp_m ?m _,
+    BD : forall _, supp_m ?m _ -> _ 
+    |- leb _ (tick _ _ ?t _ _) = true =>
+    apply BD in H; lebt t
+  end.
+Qed.
+
+Lemma time_bound `{time T} :
+  forall e C m t cf'
+         (EVAL : {|(Cf e C m t) ~> cf'|})
+         (BOUND : time_bound_ρ (Cf e C m t)),
+    time_bound_ρ cf'.
+Proof.
+  intros. remember (Cf e C m t) as cf.
+  ginduction EVAL; intros; simpl; clarify;
+  unfold time_bound_ρ in *; eauto; destruct BOUND;
+  split; try assumption;
+  match goal with
+  | RR : read ?m ?addr = Some _ |- _ =>
+    match goal with
+    | H : time_bound_m m ?t |- _ =>
+      pose proof (time_bound_read m t addr H);
+      rewrite RR in *; assumption
+    end
+  | RR : ctx_M ?C ?M = Some _ |- _ =>
+    let HINT := fresh "HINT" in
+    pose proof (time_bound_ctx_M C M) as HINT;
+    rewrite RR in HINT; apply HINT; eauto
+  | _ =>
+    repeat match goal with
+    | EVAL : {|(Cf ?e ?C ?m ?t) ~> ?cf|} |- _ =>
+      lazymatch goal with
+      | _ : leb t _ = true |- _ => fail
+      | _ => pose proof (time_increase e C m t cf EVAL); simpl in *
+      end
+    end
+  end;
+  repeat match goal with
+  | IH : forall e C m t, _ -> _ -> ?P /\ ?Q |- _ =>
+    edestruct IH; eauto;
+    match goal with
+    | _ : P |- _ => 
+      clear IH; unfold time_bound_v in *;
+      repeat des_goal; repeat des_hyp
+    | |- _ /\ _ => split;
+      match goal with
+      | |- time_bound_C ?C ?t =>
+        match goal with
+        | _ : time_bound_C C ?t' |- _ =>
+          apply relax_ctx_bound with (t1 := t'); assumption
+        end
+      | |- time_bound_m ?m ?t => assumption
+      end
+    end
+  end; subst;
+  try (edestruct IHEVAL3; eauto);
+  try (edestruct IHEVAL2; eauto);
+  repeat match goal with
+  | |- _ /\ _ => split
+  | |- time_bound_C ?C ?t =>
+    red; intros; simpl in *;
+    repeat match goal with
+    | H : _ \/ _ |- _ => destruct H; subst; try apply tick_lt
+    | _ : supp_C ?C ?t |- leb ?t _ = true =>
+      match goal with
+      | H : time_bound_C C ?t' |- _ =>
+        lebt t'; try apply H; eauto 3
+      end
+    end
+  | |- time_bound_m ?m ?t => 
+    first [assumption |
+    apply time_bound_tick; simpl; assumption]
+  end;
+  first [apply leb_refl | lebt t_a | lebt t'].
+Qed.
